WIP

src/Compilers/CommonSubexpressionEliminationWf.v
@@ -16,6 +16,9 @@ Require Import Crypto.Util.Tactics.BreakMatch.
 Require Import Crypto.Util.Tactics.DestructHead.
 Require Import Crypto.Util.Tactics.UniquePose.
 Require Import Crypto.Util.Tactics.SplitInContext.
+Require Import Crypto.Util.Option.
+Require Import Crypto.Util.Sigma.
+Require Import Crypto.Util.Prod.
 Require Import Crypto.Util.Decidable.
 
 Section symbolic.
@@ -77,11 +80,59 @@ Section symbolic.
       unfold norm_symbolize_exprf; erewrite wff_symbolize_exprf by eassumption; reflexivity.
     Qed.
 
+    Section inline.
+      Context (ctx : list symbolic_expr).
+      Fixpoint inline_symbolic_expr (s : symbolic_expr) : symbolic_expr
+        := match s with
+           | STT => STT
+           | SVar n => List.nth (List.length ctx - n) ctx (SVar n)
+           | SOp argT op args => SOp argT op (inline_symbolic_expr args)
+           | SPair x y => SPair (inline_symbolic_expr x) (inline_symbolic_expr y)
+           | SFst A B x => SFst A B (inline_symbolic_expr x)
+           | SSnd A B x => SSnd A B (inline_symbolic_expr x)
+           | SInvalid => SInvalid
+           end.
+
+      Definition inline_existT (v : { t : _ & (var1 t * symbolic_expr) * (var2 t * symbolic_expr) }%type)
+        : { t : _ & (var1 t * symbolic_expr) * (var2 t * symbolic_expr) }%type
+        := let 'existT t ((v1, s1), (v2, s2)) := v in existT _ t ((v1, inline_symbolic_expr s1), (v2, inline_symbolic_expr s2)).
+      Definition inline_ctx : list _ -> list _ := List.map inline_existT.
+
+      Lemma inline_ctx_cons x xs : inline_ctx (x :: xs) = inline_existT x :: inline_ctx xs.
+      Proof. reflexivity. Qed.
+      Lemma inline_ctx_app : forall l1 l2, inline_ctx (l1 ++ l2) = inline_ctx l1 ++ inline_ctx l2.
+      Proof. induction l1 as [|x xs IHxs], l2; simpl; rewrite ?IHxs; reflexivity. Qed.
+    End inline.
+    Global Arguments inline_existT {_} _, _ _.
+    Global Arguments inline_ctx {_} _, _ _.
+
+    Lemma In_inline {m G G'}
+          (HGG' : forall t x x', List.In (existT _ t (x, x')) G -> List.In (existT _ t (fst x, fst x')) G')
+      : forall t x x', List.In (inline_existT m (existT _ t (x, x'))) (inline_ctx m G)
+                       -> List.In (existT _ t (fst x, fst x')) G'.
+    Proof.
+      intros t x x'; specialize (fun sx sx' => HGG' t (fst x, sx) (fst x', sx')).
+      destruct x, x'; simpl in *.
+      intro H; revert dependent G'; induction G as [|g G IHG]; intros; destruct H;
+        simpl in *; unfold inline_existT in *; break_innermost_match_hyps;
+          inversion_sigma; inversion_prod; subst; simpl in *.
+      { eapply HGG'; left; reflexivity. }
+      { apply IHG; auto; [].
+        intros; eapply HGG'; right; eassumption. }
+    Qed.
+
+    Lemma map_fst_extendb {var} {c : @SymbolicExprContext (interp_flat_type var)} {t n} {v : interp_flat_type var t}
+      : map fst (extendb c n v) = n :: map fst c.
+    Proof. reflexivity. Qed.
+
     Local Arguments lookupb : simpl never.
     Local Arguments extendb : simpl never.
     Lemma wff_csef G G' t e1 e2
           (m1 : @SymbolicExprContext (interp_flat_type var1))
           (m2 : @SymbolicExprContext (interp_flat_type var2))
+          m
+          (Hm1_fst : List.map fst m1 = m)
+          (Hm2_fst : List.map fst m2 = m)
           (Hlen : length m1 = length m2)
           (Hm1m2None : forall t v, lookupb t m1 v = None <-> lookupb t m2 v = None)
           (Hm1m2Some : forall t v sv1 sv2,
@@ -92,15 +143,199 @@ Section symbolic.
                                (t:=t)
                                (symbolicify_smart_var sv1 v)
                                (symbolicify_smart_var sv2 v))
-                  -> List.In k G)
+                  -> List.In (inline_existT m k) (inline_ctx m G))
           (HG : forall t x y, List.In (existT _ t (x, y)) G -> snd x = snd y)
           (HGG' : forall t x x', List.In (existT _ t (x, x')) G -> List.In (existT _ t (fst x, fst x')) G')
           (Hwf : wff G e1 e2)
       : wff G' (@csef var1 t e1 m1) (@csef var2 t e2 m2).
     Proof.
-      revert dependent m1; revert m2; revert dependent G'.
-      induction Hwf; simpl; intros G' HGG' m2 m1 Hlen Hm1m2None Hm1m2Some; try constructor; auto.
+      subst m; revert dependent m1; revert m2; revert dependent G'.
+      induction Hwf; simpl; intros G' HGG' m2 m1 Hm1m2_fst Hlen Hm1m2None Hm1m2Some;
+        pose proof (In_inline (m:=List.map fst m2) HGG') as HGG'_inline; move HGG'_inline at top;
+          try constructor; auto.
       { erewrite wff_norm_symbolize_exprf by eassumption.
+        break_innermost_match;
+          try match goal with
+              | [ H : lookupb ?m1 ?x = Some ?k, H' : lookupb ?m2 ?x = None |- _ ]
+                => apply Hm1m2None in H'; congruence
+              end;
+          lazymatch goal with
+          | [ |- wff _ (LetIn _ _) (LetIn _ _) ]
+            => constructor; intros; auto; []
+          | _ => idtac
+          end;
+          match goal with H : _ |- _ => apply H end.
+        Set Ltac Profiling.
+        all:try solve [ repeat first [ progress intros *
+                                     | reflexivity
+                                     | progress subst
+                                     | progress inversion_option
+                                     | match goal with |- context[lookupb (extendb _ _ _) _] => idtac end;
+                                       rewrite !(fun var => @lookupb_extendb_full flat_type _ symbolic_expr _ var _ SymbolicExprContextOk)
+                                     | match goal with |- context[List.In ?k (?x ++ ?y)] => idtac end;
+                                       rewrite !in_app_iff
+                                     | rewrite !inline_ctx_app
+                                     | match goal with |- context[map fst (extendb _ _ _)] => idtac end;
+                                       rewrite !map_fst_extendb
+                                     | match goal with |- context[length (extendb _ _ _)] => idtac end;
+                                       unfold SymbolicExprContext; rewrite !length_extendb
+                                     | progress cbv beta delta [symbolize_var] in *
+                                     | progress destruct_head'_or
+                                     | progress cbn [fst snd projT1 projT2 eq_rect eq_rec eq_ind] in *
+                                     | unfold inline_ctx; solve [ auto using in_map ]
+                                     | match goal with
+                                       | [ H : map fst _ = _ |- _ ] => rewrite H
+                                       | [ H : length _ = _ |- _ ] => rewrite H
+                                       | [ H : ?x = _, H' : context[?x] |- _ ] => rewrite H in H'
+                                       | [ H : ?x <> ?x |- _ ] => exfalso; apply H; reflexivity
+                                       end
+                                     | match goal with |- _ \/ _ -> _ => idtac end;
+                                       let H := fresh in intros [H|H]; eauto; revert H; []
+                                     | progress intros
+                                     | match goal with
+                                       | [ H : List.In _ (flatten_binding_list (symbolicify_smart_var ?x1 ?v) (symbolicify_smart_var ?x2 ?v)) |- _ ]
+                                         => solve [ destruct (flatten_binding_list_SmartVarfMap2_pair_In_split H); eauto ]
+                                       | [ H : List.In _ (flatten_binding_list (symbolicify_smart_var ?x1 ?v) (symbolicify_smart_var ?x2 ?v)) |- _ ]
+                                         => exact (flatten_binding_list_SmartVarfMap2_pair_same_in_eq2 H)
+                                       end
+                                     | break_innermost_match_step
+                                     | break_innermost_match_hyps_step
+                                     | apply conj ] ].
+        all:intros *.
+        all:rewrite ?(fun var => @lookupb_extendb_full flat_type _ symbolic_expr _ var _ SymbolicExprContextOk).
+        all:try (progress break_innermost_match; subst; cbn [eq_rect eq_rec];
+                 intros ??; inversion_option; subst).
+        all:try solve [ repeat first [ progress intros *
+                           | reflexivity
+                           | progress subst
+                           | progress cbn [fst snd projT1 projT2 eq_rect eq_rec eq_ind] in *
+                           | progress inversion_option
+                           | rewrite !(fun var => @lookupb_extendb_full flat_type _ symbolic_expr _ var _ SymbolicExprContextOk)
+                           | rewrite !in_app_iff
+                           | rewrite !inline_ctx_app
+                           | rewrite !map_fst_extendb
+                           | unfold SymbolicExprContext; rewrite !length_extendb
+                           | progress unfold symbolize_var in *
+                           | progress destruct_head'_or
+                           | unfold inline_ctx; solve [ auto using in_map ]
+                           | match goal with
+                             | [ H : map fst _ = _ |- _ ] => rewrite H
+                             | [ H : length _ = _ |- _ ] => rewrite H
+                             | [ H : ?x = _, H' : context[?x] |- _ ] => rewrite H in H'
+                             | [ H : ?x <> ?x |- _ ] => exfalso; apply H; reflexivity
+                             end
+                           | match goal with |- _ \/ _ -> _ => idtac end;
+                             let H := fresh in intros [H|H]; eauto; revert H; []
+                           | progress intros
+                           | match goal with
+                             | [ H : List.In _ (flatten_binding_list (symbolicify_smart_var ?x1 ?v) (symbolicify_smart_var ?x2 ?v)) |- _ ]
+                               => solve [ destruct (flatten_binding_list_SmartVarfMap2_pair_In_split H); eauto ]
+                             | [ H : List.In _ (flatten_binding_list (symbolicify_smart_var ?x1 ?v) (symbolicify_smart_var ?x2 ?v)) |- _ ]
+                               => exact (flatten_binding_list_SmartVarfMap2_pair_same_in_eq2 H)
+                             end
+                           | break_innermost_match_step
+                           | break_innermost_match_hyps_step
+                           | apply conj
+                           | progress destruct_head'_sigT
+                           | progress destruct_head'_prod ] ].
+        Arguments inline_existT : clear implicits.
+        { induction t.
+          { simpl in *.
+            intros ? [?| [] ].
+            subst.
+            simpl.
+            rewrite inline_ctx_app.
+            rewrite in_app_iff.
+            Arguments inline_ctx : clear implicits.
+            simpl.
+        match goal with
+        | [ Hm1m2Some : forall t v sv1 sv2, lookupb ?m1 _ = _ -> lookupb ?m2 _ = _ -> forall k, _ -> _,
+              H1 : lookupb ?t' ?m1 ?v' = Some ?sv1',
+              H2 : lookupb ?t' ?m2 ?v' = Some ?sv2'
+              |- forall k', In k' _ -> _ ]
+          => let H := fresh in
+             let k := fresh k in
+             intros k H;
+               pose proof (Hm1m2Some t' v' sv1' sv2' H1 H2 k H)
+        end.
+        repeat first [ progress intros *
+                     | reflexivity
+                     | progress subst
+                     | progress cbn [fst snd projT1 projT2 eq_rect eq_rec eq_ind] in *
+                     | progress inversion_option
+                     | rewrite !(fun var => @lookupb_extendb_full flat_type _ symbolic_expr _ var _ SymbolicExprContextOk)
+                     | rewrite !in_app_iff
+                     | rewrite !inline_ctx_app
+                     | rewrite !map_fst_extendb
+                     | unfold SymbolicExprContext; rewrite !length_extendb
+                     | progress unfold symbolize_var in *
+                     | progress destruct_head'_or
+                     | unfold inline_ctx; solve [ auto using in_map ]
+                     | match goal with
+                       | [ H : map fst _ = _ |- _ ] => rewrite H
+                       | [ H : length _ = _ |- _ ] => rewrite H
+                       | [ H : ?x = _, H' : context[?x] |- _ ] => rewrite H in H'
+                       | [ H : ?x <> ?x |- _ ] => exfalso; apply H; reflexivity
+                       end
+                     | match goal with |- _ \/ _ -> _ => idtac end;
+                       let H := fresh in intros [H|H]; eauto; revert H; []
+                     | progress intros
+                     | match goal with
+                       | [ H : List.In _ (flatten_binding_list (symbolicify_smart_var ?x1 ?v) (symbolicify_smart_var ?x2 ?v)) |- _ ]
+                         => solve [ destruct (flatten_binding_list_SmartVarfMap2_pair_In_split H); eauto ]
+                       | [ H : List.In _ (flatten_binding_list (symbolicify_smart_var ?x1 ?v) (symbolicify_smart_var ?x2 ?v)) |- _ ]
+                         => exact (flatten_binding_list_SmartVarfMap2_pair_same_in_eq2 H)
+                       end
+                     | break_innermost_match_step
+                     | break_innermost_match_hyps_step
+                     | apply conj ].
+        Arguments inline_existT : clear implicits.
+          right.
+          unfold inline_existT in *.
+          admit. }
+          Set Printing Implicit.
+                           | match goal with
+                             end ] ].
+          move Hm1m2Some at bottom.
+          specialize (Hm1m2Some _ _ _ _ H3 H4).
+          intro k; specialize (Hm1m2Some k).
+          intro H'; specialize (Hm1m2Some H').
+                    { progress unfold symbolize_var in *.
+          unfold symbolize_var in *.
+
+          left; apply Hm1m2Some.
+          { .
+          { auto.
+          a
+                           | apply conj ].
+          move m1 at bottom.
+          match goal with
+
+          2:reflexivity.
+          Show Ltac Profile.
+          Focus 2.
+          move x1 at bottom.
+          Focus 2.
+          Show Ltac Profile.
+          all:try match goal with
+                         | [ H : List.In _ (flatten_binding_list (symbolicify_smart_var ?x1 ?v) (symbolicify_smart_var ?x2 ?v)) |- _ ]
+                           => solve [ destruct (flatten_binding_list_SmartVarfMap2_pair_In_split H); eauto ]
+                  end.
+          SearchAbout flatten_binding_list symbolicify_smart_var.
+
+          solve [ unfold inline_ctx; eauto using in_map ].
+
+          |
+          unfold symbolize_var.
+          Print symbolize_var.
+          Focus 4.
+          unfold extendb; simpl.
+          Check @extendb.
+                                              .
+                           | rewrite].
+          all:intros *.
+          all:
+          intros; apply H0; eauto.
         break_innermost_match;
           try match goal with
               | [ H : lookupb ?m1 ?x = Some ?k, H' : lookupb ?m2 ?x = None |- _ ]
@@ -115,10 +350,121 @@ Section symbolic.
           try solve [ repeat first [ progress unfold symbolize_var
                        | rewrite Hlen
                        | progress subst
+                       | progress inversion_option
                        | setoid_rewrite length_extendb
+                       | setoid_rewrite List.in_app_iff
+                       | setoid_rewrite inline_ctx_app
+                       | setoid_rewrite inline_ctx_cons
+                       | progress destruct_head' or
+                       | solve [ unfold inline_ctx; eauto using in_map ]
+                       | progress intros
+                       | match goal with
+                         | [ H : List.In _ (flatten_binding_list (symbolicify_smart_var ?x1 ?v) (symbolicify_smart_var ?x2 ?v)) |- _ ]
+                           => solve [ destruct (flatten_binding_list_SmartVarfMap2_pair_In_split H); eauto ]
+                         | [ H : List.In _ (flatten_binding_list (symbolicify_smart_var ?x1 ?v) (symbolicify_smart_var ?x2 ?v)) |- _ ]
+                           => exact (flatten_binding_list_SmartVarfMap2_pair_same_in_eq2 H)
+                         | [ H : context[lookupb (extendb _ _ _) _] |- _ ]
+                           => rewrite (fun var => @lookupb_extendb_full flat_type _ symbolic_expr _ var _ SymbolicExprContextOk) in H
+                         end
+                       | rewrite !(fun var => @lookupb_extendb_full flat_type _ symbolic_expr _ var _ SymbolicExprContextOk)
+                       | break_innermost_match_step
+                       | break_innermost_match_hyps_step
+                       | progress simpl in *
+                       | solve [ intuition (eauto || congruence) ]
+                       | match goal with
+                         | [ H : forall t x y, _ |- _ ] => specialize (fun t x0 x1 y0 y1 => H t (x0, x1) (y0, y1)); cbn [fst snd] in H
+                         | [ H : In (existT _ ?t (?x, ?x')) (flatten_binding_list (symbolicify_smart_var _ _) (symbolicify_smart_var _ _)),
+                                 Hm1m2Some : forall t v sv1 sv2, _ -> _ -> forall k', In k' (flatten_binding_list _ _) -> In (inline_existT k') (inline_ctx ?G) |- _ ]
+                           => is_var x; is_var x';
+                              lazymatch goal with
+                              | [ H : In (existT _ t ((fst x, _), (fst x', _))) G |- _ ] => fail
+                              | _ => let H' := fresh in
+                                     refine (let H' := flatten_binding_list_SmartVarfMap2_pair_in_generalize2 H _ _ in _);
+                                     destruct H' as [? [? H']];
+                                     eapply Hm1m2Some in H'; [ | eassumption.. ]
+                              end
+                         end ] ].
+        { repeat first [ progress unfold symbolize_var
+                       | rewrite Hlen
+                       | progress subst
+                       | progress inversion_option
+                       | setoid_rewrite length_extendb
+                       | setoid_rewrite List.in_app_iff
+                       | setoid_rewrite inline_ctx_app
+                       | setoid_rewrite inline_ctx_cons
+                       | progress destruct_head' or
+                       | solve [ unfold inline_ctx; eauto using in_map ]
+                       | progress intros
+                       | match goal with
+                         | [ H : List.In _ (flatten_binding_list (symbolicify_smart_var ?x1 ?v) (symbolicify_smart_var ?x2 ?v)) |- _ ]
+                           => solve [ destruct (flatten_binding_list_SmartVarfMap2_pair_In_split H); eauto ]
+                         | [ H : List.In _ (flatten_binding_list (symbolicify_smart_var ?x1 ?v) (symbolicify_smart_var ?x2 ?v)) |- _ ]
+                           => exact (flatten_binding_list_SmartVarfMap2_pair_same_in_eq2 H)
+                         | [ H : context[lookupb (extendb _ _ _) _] |- _ ]
+                           => rewrite (fun var => @lookupb_extendb_full flat_type _ symbolic_expr _ var _ SymbolicExprContextOk) in H
+                         end
+                       | rewrite !(fun var => @lookupb_extendb_full flat_type _ symbolic_expr _ var _ SymbolicExprContextOk)
+                       | break_innermost_match_step
+                       | break_innermost_match_hyps_step
+                       | progress simpl in *
+                       | solve [ intuition (eauto || congruence) ]
+                       | match goal with
+                         | [ H : forall t x y, _ |- _ ] => specialize (fun t x0 x1 y0 y1 => H t (x0, x1) (y0, y1)); cbn [fst snd] in H
+                         | [ H : In (existT _ ?t (?x, ?x')) (flatten_binding_list (symbolicify_smart_var _ _) (symbolicify_smart_var _ _)),
+                                 Hm1m2Some : forall t v sv1 sv2, _ -> _ -> forall k', In k' (flatten_binding_list _ _) -> In (inline_existT k') (inline_ctx ?G) |- _ ]
+                           => is_var x; is_var x';
+                              lazymatch goal with
+                              | [ H : In (existT _ t ((fst x, _), (fst x', _))) G |- _ ] => fail
+                              | _ => let H' := fresh in
+                                     refine (let H' := flatten_binding_list_SmartVarfMap2_pair_in_generalize2 H _ _ in _);
+                                     destruct H' as [? [? H']];
+                                     eapply Hm1m2Some in H'; [ | eassumption.. ]
+                              end
+                         end ].
+          { eapply HGG'_inline.
+        {          repeat first [ progress unfold symbolize_var
+                       | rewrite Hlen
+                       | progress subst
+                       | setoid_rewrite length_extendb
+                       | setoid_rewrite inline_ctx_app
+                       | setoid_rewrite inline_ctx_cons
                        | setoid_rewrite List.in_app_iff
                        | progress destruct_head' or
                        | solve [ eauto ]
+                       | progress intros ].
+                   repeat match goal with
+                          | [ H : forall t x y, _ |- _ ] => specialize (fun t x0 x1 y0 y1 => H t (x0, x1) (y0, y1)); cbn [fst snd] in H
+                          end.
+                   { lazymatch goal with
+                     end.
+                     eauto.
+
+                   unfold fst; break_innermost_match.
+                   eapply (HGG'_inline _ (_, _) (_, _)).
+                   move G at bottom.
+                   match goal with
+                   | [ H : forall
+                   eapply (fun H1 H2 => Hm1m2Some _ _ _ _ H1 H2 (existT _ _ ((_, _), (_, _)))).
+                   eauto.
+                   match goal with
+                   | [ H : List.In _ (flatten_binding_list (symbolicify_smart_var ?x1 ?v) (symbolicify_smart_var ?x2 ?v)) |- _ ]
+                     => destruct (flatten_binding_list_SmartVarfMap2_pair_In_split H); eauto
+                   end.
+                   move G' at bottom.
+
+
+        { repeat first
+        Focus 7.
+        { repeat first [ progress unfold symbolize_var
+                       | rewrite Hlen
+                       | progress subst
+                       | progress inversion_option
+                       | setoid_rewrite length_extendb
+                       | setoid_rewrite List.in_app_iff
+                       | setoid_rewrite inline_ctx_app
+                       | setoid_rewrite inline_ctx_cons
+                       | progress destruct_head' or
+                       | solve [ unfold inline_ctx; eauto using in_map ]
                        | progress intros
                        | match goal with
                          | [ H : List.In _ (flatten_binding_list (symbolicify_smart_var ?x1 ?v) (symbolicify_smart_var ?x2 ?v)) |- _ ]
@@ -145,7 +491,125 @@ Section symbolic.
                                      destruct H' as [? [? H']];
                                      eapply Hm1m2Some in H'; [ | eassumption.. ]
                               end
-                         end ] ].
+                         end ].
+          { destruct_head'_sigT.
+            destruct_head'_prod.
+        { repeat first [ progress unfold symbolize_var
+                       | rewrite Hlen
+                       | progress subst
+                       | progress inversion_option
+                       | setoid_rewrite length_extendb
+                       | setoid_rewrite List.in_app_iff
+                       | setoid_rewrite inline_ctx_app
+                       | setoid_rewrite inline_ctx_cons
+                       | progress destruct_head' or
+                       | solve [ unfold inline_ctx; eauto using in_map ]
+                       | progress intros
+                       | match goal with
+                         | [ H : List.In _ (flatten_binding_list (symbolicify_smart_var ?x1 ?v) (symbolicify_smart_var ?x2 ?v)) |- _ ]
+                           => solve [ destruct (flatten_binding_list_SmartVarfMap2_pair_In_split H); eauto ]
+                         | [ H : List.In _ (flatten_binding_list (symbolicify_smart_var ?x1 ?v) (symbolicify_smart_var ?x2 ?v)) |- _ ]
+                           => exact (flatten_binding_list_SmartVarfMap2_pair_same_in_eq2 H)
+                         | [ H : context[lookupb (extendb _ _ _) _] |- _ ]
+                           => rewrite (fun var => @lookupb_extendb_full flat_type _ symbolic_expr _ var _ SymbolicExprContextOk) in H
+                         end
+                       | rewrite !(fun var => @lookupb_extendb_full flat_type _ symbolic_expr _ var _ SymbolicExprContextOk)
+                       | break_innermost_match_step
+                       | break_innermost_match_hyps_step
+                       | progress simpl in *
+                       | solve [ intuition (eauto || congruence) ]
+                       | match goal with
+                         | [ H : forall t x y, _ |- _ ] => specialize (fun t x0 x1 y0 y1 => H t (x0, x1) (y0, y1)); cbn [fst snd] in H
+                         | [ H : In (existT _ ?t (?x, ?x')) (flatten_binding_list (symbolicify_smart_var _ _) (symbolicify_smart_var _ _)),
+                                 Hm1m2Some : forall t v sv1 sv2, _ -> _ -> forall k', In k' (flatten_binding_list _ _) -> In k' ?G |- _ ]
+                           => is_var x; is_var x';
+                              lazymatch goal with
+                              | [ H : In (existT _ t ((fst x, _), (fst x', _))) G |- _ ] => fail
+                              | _ => let H' := fresh in
+                                     refine (let H' := flatten_binding_list_SmartVarfMap2_pair_in_generalize2 H _ _ in _);
+                                     destruct H' as [? [? H']];
+                                     eapply Hm1m2Some in H'; [ | eassumption.. ]
+                              end
+                         end ].
+          lazymatch goal with
+            | [ H : List.In _ (flatten_binding_list (symbolicify_smart_var ?x1 ?v) (symbolicify_smart_var ?x2 ?v)) |- _ ]
+              => destruct (flatten_binding_list_SmartVarfMap2_pair_In_split H); eauto
+            end.
+          left.
+        { repeat first [ progress unfold symbolize_var
+                       | rewrite Hlen
+                       | progress subst
+                       | progress inversion_option
+                       | setoid_rewrite length_extendb
+                       | setoid_rewrite List.in_app_iff
+                       | setoid_rewrite inline_ctx_app
+                       | setoid_rewrite inline_ctx_cons
+                       | progress destruct_head' or
+                       | solve [ unfold inline_ctx; eauto using in_map ]
+                       | progress intros
+                       | match goal with
+                         | [ H : List.In _ (flatten_binding_list (symbolicify_smart_var ?x1 ?v) (symbolicify_smart_var ?x2 ?v)) |- _ ]
+                           => solve [ destruct (flatten_binding_list_SmartVarfMap2_pair_In_split H); eauto ]
+                         | [ H : List.In _ (flatten_binding_list (symbolicify_smart_var ?x1 ?v) (symbolicify_smart_var ?x2 ?v)) |- _ ]
+                           => exact (flatten_binding_list_SmartVarfMap2_pair_same_in_eq2 H)
+                         | [ H : context[lookupb (extendb _ _ _) _] |- _ ]
+                           => rewrite (fun var => @lookupb_extendb_full flat_type _ symbolic_expr _ var _ SymbolicExprContextOk) in H
+                         end
+                       | rewrite !(fun var => @lookupb_extendb_full flat_type _ symbolic_expr _ var _ SymbolicExprContextOk)
+                       | break_innermost_match_step
+                       | break_innermost_match_hyps_step
+                       | progress simpl in *
+                       | solve [ intuition (eauto || congruence) ]
+                       | match goal with
+                         | [ H : forall t x y, _ |- _ ] => specialize (fun t x0 x1 y0 y1 => H t (x0, x1) (y0, y1)); cbn [fst snd] in H
+                         | [ H : In (existT _ ?t (?x, ?x')) (flatten_binding_list (symbolicify_smart_var _ _) (symbolicify_smart_var _ _)),
+                                 Hm1m2Some : forall t v sv1 sv2, _ -> _ -> forall k', In k' (flatten_binding_list _ _) -> In k' ?G |- _ ]
+                           => is_var x; is_var x';
+                              lazymatch goal with
+                              | [ H : In (existT _ t ((fst x, _), (fst x', _))) G |- _ ] => fail
+                              | _ => let H' := fresh in
+                                     refine (let H' := flatten_binding_list_SmartVarfMap2_pair_in_generalize2 H _ _ in _);
+                                     destruct H' as [? [? H']];
+                                     eapply Hm1m2Some in H'; [ | eassumption.. ]
+                              end
+                         end ].
+          lazymatch goal with
+          | [ H : In (existT _ ?t (?x, ?x')) (flatten_binding_list (symbolicify_smart_var _ _) (symbolicify_smart_var _ _)),
+                  Hm1m2Some : forall t v sv1 sv2, _ -> _ -> forall k', In k' (flatten_binding_list _ _) -> In (inline_existT k') (inline_ctx ?G) |- _ ]
+            => idtac end.
+            => is_var x; is_var x';
+                 lazymatch goal with
+                 | [ H : In (existT _ t ((fst x, _), (fst x', _))) G |- _ ] => fail
+                 | _ => let H' := fresh in
+                        refine (let H' := flatten_binding_list_SmartVarfMap2_pair_in_generalize2 H _ _ in _);
+                          destruct H' as [? [? H']];
+                          eapply Hm1m2Some in H'; [ | eassumption.. ]
+                 end
+          end.
+          lazymatch goal with
+          | [ H : In (existT _ ?t (?x, ?x')) (flatten_binding_list (symbolicify_smart_var _ _) (symbolicify_smart_var _ _)),
+                  Hm1m2Some : forall t v sv1 sv2, _ -> _ -> forall k', In k' (flatten_binding_list _ _) -> In k' ?G |- _ ]
+            => is_var x; is_var x';
+                 lazymatch goal with
+                 | [ H : In (existT _ t ((fst x, _), (fst x', _))) G |- _ ] => fail
+                 | _ => let H' := fresh in
+                        refine (let H' := flatten_binding_list_SmartVarfMap2_pair_in_generalize2 H _ _ in _);
+                          destruct H' as [? [? H']];
+                          eapply Hm1m2Some in H'; [ | eassumption.. ]
+                 end
+          end.
+lazymatch goal with
+                         | [ H : List.In _ (flatten_binding_list (symbolicify_smart_var ?x1 ?v) (symbolicify_smart_var ?x2 ?v)) |- _ ]
+                           => destruct (flatten_binding_list_SmartVarfMap2_pair_In_split H); eauto
+end.
+eauto.
+
+                         | [ H : List.In _ (flatten_binding_list (symbolicify_smart_var ?x1 ?v) (symbolicify_smart_var ?x2 ?v)) |- _ ]
+                           => exact (flatten_binding_list_SmartVarfMap2_pair_same_in_eq2 H)
+                         | [ H : context[lookupb (extendb _ _ _) _] |- _ ]
+                           => rewrite (fun var => @lookupb_extendb_full flat_type _ symbolic_expr _ var _ SymbolicExprContextOk) in H
+                         end          .
+          SearchAbout (In (?f ?x) (List.map ?f ?ls)).
          repeat first [ progress unfold symbolize_var
                        | rewrite Hlen
                        | progress subst
@@ -154,6 +618,20 @@ Section symbolic.
                        | progress destruct_head' or
                        | solve [ eauto ]
                        | progress intros ].
+         repeat match goal with
+                | [ H : context[lookupb (extendb _ _ _) _] |- _ ]
+                  => rewrite (fun var => @lookupb_extendb_full flat_type _ symbolic_expr _ var _ SymbolicExprContextOk) in H
+                end.
+
+         break_innermost_match_hyps; subst; cbn [eq_rect eq_rec eq_ind] in *; inversion_option; subst; auto.
+
+         Focus 2.
+
+         Check symbolicify_smart_var.
+         left; assumption.
+        end
+         pose (@lookupb_extendb_full _ base_type_code_dec).
+         rewrite (@lookupb_extendb_full in H1.
          (** FIXME: This actually isn't true, because the symbolic
              expr stored in G might not be the same as the one in the
              expression tree, when the one in the expression tree is a
