src/Compilers/CommonSubexpressionEliminationInterp.v
@@ -1,5 +1,6 @@
 (** * Common Subexpression Elimination for PHOAS Syntax *)
 Require Import Coq.Lists.List.
+Require Import Coq.omega.Omega.
 Require Import Crypto.Compilers.Named.Context.
 Require Import Crypto.Compilers.Named.AListContext.
 Require Import Crypto.Compilers.Named.ContextDefinitions.
@@ -13,7 +14,7 @@ Require Import Crypto.Compilers.WfProofs.
 Require Import Crypto.Compilers.SmartMap.
 Require Import Crypto.Compilers.CommonSubexpressionElimination.
 Require Import Crypto.Compilers.CommonSubexpressionEliminationDenote.
-Require Import Crypto.Compilers.CommonSubexpressionEliminationWf.
+(*Require Import Crypto.Compilers.CommonSubexpressionEliminationWf.*)
 Require Import Crypto.Util.Bool.
 Require Import Crypto.Util.Tactics.RewriteHyp.
 Require Import Crypto.Util.Tactics.BreakMatch.
@@ -24,6 +25,7 @@ Require Import Crypto.Util.Prod.
 Require Import Crypto.Util.Option.
 Require Import Crypto.Util.Sigma.
 Require Import Crypto.Util.Decidable.
+Require Import Crypto.Util.HProp.
 
 Section symbolic.
   Context (base_type_code : Type)
@@ -67,6 +69,13 @@ Section symbolic.
 
   Local Notation denote_symbolic_expr := (@denote_symbolic_expr base_type_code op_code base_type_code_beq op_code_beq base_type_code_bl op denote_op interp_base_type interp_op).
 
+  Local Notation norm_symbolize_exprf := (@norm_symbolize_exprf base_type_code op_code op symbolize_op normalize_symbolic_op_arguments).
+
+  Context (denote_symbolic_expr_normalize
+           : forall t m e, denote_symbolic_expr m t (symbolic_expr_normalize base_type_code op_code normalize_symbolic_op_arguments e) = denote_symbolic_expr m t e).
+  Context (denote_symbolize_op
+           : forall s d opc, denote_op s d (symbolize_op s d opc) = Some opc).
+
   Local Instance base_type_code_dec : DecidableRel (@eq base_type_code)
     := dec_rel_of_bool_dec_rel base_type_code_beq base_type_code_bl base_type_code_lb.
   Local Instance op_code_dec : DecidableRel (@eq op_code)
@@ -87,6 +96,57 @@ Section symbolic.
                    | rewrite List.in_app_iff in *
                    | progress intros
                    | solve [ eauto ] ].
+  Qed.
+
+  Lemma denote_symbolic_expr_flatten_binding_list T t x y v s m
+        (Hm : forall t sv v,
+            lookupb m sv = Some v
+            -> denote_symbolic_expr m t sv = Some v)
+        (Heq : denote_symbolic_expr m T s = Some v)
+        (H : List.In (existT _ t (x, y)) (flatten_binding_list (var2:=interp_base_type) (t:=T) (symbolicify_smart_var v s) v))
+    : denote_symbolic_expr m (Tbase t) (snd x) = Some y.
+  Proof.
+    revert dependent s; induction T;
+      try solve [ repeat first [ progress simpl in *
+                               | reflexivity
+                               | tauto
+                               | progress destruct_head or
+                               | progress inversion_sigma
+                               | progress inversion_prod
+                               | progress inversion_option
+                               | progress subst
+                               | rewrite List.in_app_iff in *
+                               | progress intros
+                               | progress cbn [fst snd projT1 projT2] in *
+                               | solve [ eauto ]
+                               | break_innermost_match_hyps_step
+                               | unfold var_cast in *;
+                                 break_innermost_match_hyps;
+                                 [ lazymatch goal with
+                                   | [ H : context[match eq_trans ?p (eq_sym ?q) with _ => _ end] |- _ ]
+                                     => revert H; generalize p; generalize (eq_sym q); intros
+                                   end
+                                 | discriminate.. ]
+                               | progress eliminate_hprop_eq
+                               | progress destruct_head'_prod
+                               | progress destruct_head'_sigT ] ].
+    { intro s;
+        specialize (IHT1 (fst v) (SFst T1 T2 s));
+        specialize (IHT2 (snd v) (SSnd T1 T2 s)).
+      repeat first [ progress cbn [denote_symbolic_expr option_map] in *
+                   | progress break_innermost_match_hyps_step
+                   | discriminate
+                   | match goal with
+                     | [ H : context[flat_type_beq _ _ ?x ?x] |- _ ]
+                       => setoid_rewrite (flat_type_dec_lb _ _ base_type_code_lb x x eq_refl) in H
+                     | [ H : ?x = Some _, H' : context[?x] |- _ ] => rewrite H in H'
+                     end
+                   | progress specialize_by reflexivity
+                   | progress intros
+                   | progress simpl in *
+                   | rewrite in_app_iff in *
+                   | progress destruct_head'_or
+                   | solve [ eauto ] ]. }
   Qed.
 
   (*Lemma interpf_symbolize_exprf_injective
@@ -130,15 +190,97 @@ Section symbolic.
     move s at top; reverse.
                 ->
 
-*)
+   *)
 
+  Lemma denote_symbolic_expr_symbolize_exprf {t G e e' s}
+        (HG : forall t x y, In (existT _ t (x, y)) G -> fst x = y)
+        (m : @SymbolicExprContext (interp_flat_type_gen _))
+        (HGm : forall t s v,
+            lookupb m s = Some v
+            -> forall k,
+              List.In k (flatten_binding_list (@symbolicify_smart_var interp_base_type t v s) v)
+              -> List.In k G)
+        (HG2 : forall t x y, In (existT _ t (x, y)) G -> denote_symbolic_expr m (Tbase _) (snd x) = Some y)
+        (Hm : forall t sv v,
+            lookupb m sv = Some v
+            -> denote_symbolic_expr m t sv = Some v)
+        (Hwf : wff G e e')
+        (Heq : @symbolize_exprf interp_base_type t e = Some s)
+    : denote_symbolic_expr m t s = Some (interpf interp_op e').
+  Proof.
+    cbv beta in *.
+    revert dependent m; revert dependent s;
+      induction Hwf; simpl; cbv [LetIn.Let_In symbolize_var]; intros; eauto;
+        rewrite_hyp ?* by eauto; try reflexivity; eauto;
+          cbn [symbolize_exprf option_map] in *;
+          repeat first [ reflexivity
+                       | progress subst
+                       | progress inversion_option
+                       | progress cbn [symbolize_exprf] in *
+                       | progress unfold option_map in *
+                       | break_innermost_match_hyps_step
+                       | rewrite denote_symbolize_op in *
+                       | progress cbn [denote_symbolic_expr] in *
+                       | break_innermost_match_step
+                       | progress specialize_by_assumption
+                       | solve [ eauto ]
+                       | match goal with
+                         | [ H : ?v = Some ?x |- Some (interp_op ?s ?d ?opc ?x) = Some (interp_op ?s ?d ?opc ?y) ]
+                           => is_var x; cut (v = Some y); [ congruence | clear x H ]
+                         | [ H1 : ?v1 = Some ?x1, H2 : ?v2 = Some ?x2 |- Some (?x1, ?x2) = Some (?k1, ?k2) ]
+                           => is_var x1; is_var x2; cut (v1 = Some k1 /\ v2 = Some k2);
+                              [ clear -H1 H2; intros [? ?]; congruence | clear x1 x2 H1 H2; split ]
+                         | [ H : forall x, Some x = Some _ -> _ |- _ ] => specialize (H _ eq_refl)
+                         | [ H : forall x, Some _ = Some x -> _ |- _ ] => specialize (H _ eq_refl)
+                         | [ IHHwf : _, H : denote_symbolic_expr _ _ _ = None |- _ ]
+                           => rewrite IHHwf in H by eauto; discriminate
+                         end ].
+  Qed.
 
+  Lemma denote_symbolic_expr_norm_symbolize_exprf {t G e e' s}
+        (Heq : @norm_symbolize_exprf interp_base_type t e = Some s)
+        (m : @SymbolicExprContext (interp_flat_type_gen _))
+        (HG : forall t x y, In (existT _ t (x, y)) G -> fst x = y)
+        (HGm : forall t s v,
+            lookupb m s = Some v
+            -> forall k,
+              List.In k (flatten_binding_list (@symbolicify_smart_var interp_base_type t v s) v)
+              -> List.In k G)
+        (HG2 : forall t x y, In (existT _ t (x, y)) G -> denote_symbolic_expr m (Tbase _) (snd x) = Some y)
+        (Hm : forall t sv v,
+            lookupb m sv = Some v
+            -> denote_symbolic_expr m t sv = Some v)
+        (Hwf : wff G e e')
+    : denote_symbolic_expr m t s = Some (interpf interp_op e').
+  Proof.
+    unfold norm_symbolize_exprf, option_map in Heq.
+    destruct (symbolize_exprf e) eqn:Heq'; inversion_option; subst.
+    rewrite denote_symbolic_expr_normalize.
+    eapply denote_symbolic_expr_symbolize_exprf; eauto.
+  Qed.
+
+  Local Notation context_equiv := (@context_equiv _ _ _ (@SymbolicExprContext interp_flat_type)).
+  Require Import Coq.Classes.Morphisms.
+  Axiom denote_symbolic_expr_Proper : Proper (context_equiv ==> forall_relation (fun t => eq ==> eq)) denote_symbolic_expr.
+  Axiom denote_symbolic_expr_weaken
+    : forall c1 c2,
+      (forall t n v, lookupb t c1 n = Some v -> lookupb t c2 n = Some v)
+      -> forall t sv v,
+        denote_symbolic_expr c1 t sv = Some v
+        -> denote_symbolic_expr c2 t sv = Some v.
+  Axiom denote_symbolic_expr_two_types
+    : forall m t0 t1 s,
+      denote_symbolic_expr m t0 s <> None
+      -> denote_symbolic_expr m t1 s <> None
+      -> t0 = t1.
 
   Local Arguments lookupb : simpl never.
   Local Arguments extendb : simpl never.
   Lemma interpf_csef G t e1 e2
-        (HG : forall t x y, In (existT _ t (x, y)) G -> fst x = y)
         (m : @SymbolicExprContext (interp_flat_type_gen _))
+        (Hwf : wff G e1 e2)
+        (HG : forall t x y, In (existT _ t (x, y)) G -> fst x = y)
+        (HG2 : forall t x y, In (existT _ t (x, y)) G -> denote_symbolic_expr m (Tbase _) (snd x) = Some y)
         (HGm : forall t s v,
             lookupb m s = Some v
             -> forall k,
@@ -147,15 +289,1553 @@ Section symbolic.
         (Hm : forall t sv v,
             lookupb m sv = Some v
             -> denote_symbolic_expr m t sv = Some v)
-        (Hwf : wff G e1 e2)
     : interpf interp_op (@csef interp_base_type t e1 m) = interpf interp_op e2.
   Proof.
     cbv beta in *.
       revert dependent m;
         induction Hwf; simpl; cbv [LetIn.Let_In symbolize_var]; intros; eauto;
           rewrite_hyp ?* by eauto; try reflexivity; eauto.
-      (*{ break_match; break_match_hyps; try congruence; inversion_prod; inversion_option; subst;
-          simpl; unfold LetIn.Let_In;
+      { break_innermost_match_step; [ | admit ].
+        break_innermost_match_step; [ | admit ].
+        lazymatch goal with
+        | [ H : norm_symbolize_exprf _ = Some _ |- _ ]
+          => let H' := fresh in
+             refine (let H' := denote_symbolic_expr_norm_symbolize_exprf H _ in _); clearbody H';
+               specialize_by eauto;
+               move H' at top
+        end.
+        break_innermost_match_step;
+          cbn [interpf interpf_step LetIn.Let_In];
+          try erewrite_hyp * by eauto.
+        all:match goal with
+            | [ H : _ |- _ ] => apply H
+            end.
+        all:repeat setoid_rewrite length_extendb.
+        all:try solve [ repeat first [ progress subst
+                                     | progress inversion_option
+                                     | progress intros *
+                                     | progress cbn [eq_rect eq_rec eq_ind]
+                                     | solve [ eauto using interpf_flatten_binding_list, denote_symbolic_expr_flatten_binding_list ]
+                                     | progress destruct_head'_or
+                                     | rewrite !(fun var => @lookupb_extendb_full flat_type _ symbolic_expr _ var _ SymbolicExprContextOk)
+                                     | setoid_rewrite in_app_iff
+                                     | break_innermost_match_step
+                                     | progress simpl in *
+                                     | discriminate
+                                     | assumption
+                                     | symmetry; assumption
+                                     | reflexivity
+                                     | progress intros
+                                     | match goal with
+                                       | [ H : ?x = Some ?a, H' : ?x = Some ?b |- _ ]
+                                         => assert (a = b) by (clear -H H'; congruence);
+                                            (subst a || subst b)
+                                       | [ H : ?x <> ?x |- _ ] => exfalso; apply H; clear
+                                       | [ H : lookupb ?t ?m ?n = Some _ |- None = @lookupb _ _ _ ?C ?t' ?m ?n ]
+                                         => let H' := fresh in
+                                            let RHS := match goal with |- _ = ?RHS => RHS end in
+                                            destruct RHS eqn:H'; [ | reflexivity ]
+                                       | [ Hm_small : forall t k, length ?m <= k -> lookupb ?m (SVar k) = None, H : lookupb ?m (SVar ?k') = Some _ |- _ ]
+                                         => rewrite Hm_small in H by omega
+                                       | [ Hm_small : forall t k, length ?m <= k -> lookupb ?m (SVar k) = None |- context[lookupb ?m (SVar ?k')] ]
+                                         => rewrite Hm_small by omega
+                                       | [ H : lookupb ?t ?m ?n = Some _, H' : lookupb ?t' ?m ?n = Some _ |- _ ]
+                                         => let H'' := fresh in
+                                            pose proof (@lookupb_unique_type _ _ _ _ SymbolicExprContextOk m n t t') as H'';
+                                            rewrite H, H' in H'';
+                                            specialize_by congruence;
+                                            (subst t || subst t')
+                                       | [ H : lookupb ?m ?s = Some ?k, H' : denote_symbolic_expr ?m _ ?s = Some ?k', Hm : forall t sv v, lookupb ?m sv = Some v -> denote_symbolic_expr ?m t sv = Some v |- _ ]
+                                         => let H'' := fresh in
+                                            pose proof (Hm _ _ _ H) as H'';
+                                            rewrite H' in H''; inversion_option;
+                                            (subst k || subst k')
+                                       | [ H : lookupb ?t ?m ?s = Some ?k, H' : denote_symbolic_expr ?m ?t' ?s = Some ?k', Hm : forall T sv v, lookupb ?m sv = Some v -> denote_symbolic_expr ?m T sv = Some v |- _ ]
+                                         => let H'' := fresh in
+                                            let H''' := fresh in
+                                            pose proof (Hm _ _ _ H) as H'';
+                                            pose proof (denote_symbolic_expr_two_types m t t' s) as H''';
+                                            rewrite H', H'' in H''';
+                                            specialize_by congruence;
+                                            (subst t || subst t')
+                                       | [ |- denote_symbolic_expr ?m ?t ?e = Some ?v ]
+                                         => lazymatch m with
+                                            | extendb ?m' _ _
+                                              => apply (fun pf1 => denote_symbolic_expr_weaken m' m pf1 t e v); [ intros ??? | ]
+                                            end
+                                       end ] ]. }
+      Grab Existential Variables.
+      { cbn [interpf interpf_step LetIn.Let_In];
+          try erewrite_hyp * by eauto.
+        clear Heqo.
+        all:match goal with
+            | [ H : _ |- _ ] => apply H
+            end.
+        all:try solve [ repeat first [ progress subst
+                                     | progress inversion_option
+                                     | progress intros *
+                                     | progress cbn [eq_rect eq_rec eq_ind]
+                                     | solve [ eauto using interpf_flatten_binding_list, denote_symbolic_expr_flatten_binding_list ]
+                                     | progress destruct_head'_or
+                                     | rewrite !(fun var => @lookupb_extendb_full flat_type _ symbolic_expr _ var _ SymbolicExprContextOk)
+                                     | setoid_rewrite in_app_iff
+                                     | break_innermost_match_step
+                                     | progress simpl in *
+                                     | discriminate
+                                     | assumption
+                                     | symmetry; assumption
+                                     | reflexivity
+                                     | progress intros
+                                     | match goal with
+                                       | [ H : ?x = Some ?a, H' : ?x = Some ?b |- _ ]
+                                         => assert (a = b) by (clear -H H'; congruence);
+                                            (subst a || subst b)
+                                       | [ H : ?x <> ?x |- _ ] => exfalso; apply H; clear
+                                       | [ H : lookupb ?t ?m ?n = Some _ |- None = @lookupb _ _ _ ?C ?t' ?m ?n ]
+                                         => let H' := fresh in
+                                            let RHS := match goal with |- _ = ?RHS => RHS end in
+                                            destruct RHS eqn:H'; [ | reflexivity ]
+                                       | [ Hm_small : forall t k, length ?m <= k -> lookupb ?m (SVar k) = None, H : lookupb ?m (SVar ?k') = Some _ |- _ ]
+                                         => rewrite Hm_small in H by omega
+                                       | [ Hm_small : forall t k, length ?m <= k -> lookupb ?m (SVar k) = None |- context[lookupb ?m (SVar ?k')] ]
+                                         => rewrite Hm_small by omega
+                                       | [ H : lookupb ?t ?m ?n = Some _, H' : lookupb ?t' ?m ?n = Some _ |- _ ]
+                                         => let H'' := fresh in
+                                            pose proof (@lookupb_unique_type _ _ _ _ SymbolicExprContextOk m n t t') as H'';
+                                            rewrite H, H' in H'';
+                                            specialize_by congruence;
+                                            (subst t || subst t')
+                                       | [ H : lookupb ?m ?s = Some ?k, H' : denote_symbolic_expr ?m _ ?s = Some ?k', Hm : forall t sv v, lookupb ?m sv = Some v -> denote_symbolic_expr ?m t sv = Some v |- _ ]
+                                         => let H'' := fresh in
+                                            pose proof (Hm _ _ _ H) as H'';
+                                            rewrite H' in H''; inversion_option;
+                                            (subst k || subst k')
+                                       | [ H : lookupb ?t ?m ?s = Some ?k, H' : denote_symbolic_expr ?m ?t' ?s = Some ?k', Hm : forall T sv v, lookupb ?m sv = Some v -> denote_symbolic_expr ?m T sv = Some v |- _ ]
+                                         => let H'' := fresh in
+                                            let H''' := fresh in
+                                            pose proof (Hm _ _ _ H) as H'';
+                                            pose proof (denote_symbolic_expr_two_types m t t' s) as H''';
+                                            rewrite H', H'' in H''';
+                                            specialize_by congruence;
+                                            (subst t || subst t')
+                                       | [ |- denote_symbolic_expr ?m ?t ?e = Some ?v ]
+                                         => lazymatch m with
+                                            | extendb ?m' _ _
+                                              => apply (fun pf1 => denote_symbolic_expr_weaken m' m pf1 t e v); [ intros ??? | ]
+                                            end
+                                       end ] ].
+        all:try (setoid_rewrite in_app_iff; intros; destruct_head'_or).
+        all:intros;match goal with
+        | [ |- denote_symbolic_expr ?m ?t ?e = Some ?v ]
+          => lazymatch m with
+             | extendb ?m' _ _
+               => apply (fun pf1 => denote_symbolic_expr_weaken m' m pf1 t e v); [ intros ??? | ]
+             end
+        end.
+        all:try solve [ repeat first [ progress subst
+                                     | progress inversion_option
+                                     | progress intros *
+                                     | progress cbn [eq_rect eq_rec eq_ind]
+                                     | solve [ eauto using interpf_flatten_binding_list, denote_symbolic_expr_flatten_binding_list ]
+                                     | progress destruct_head'_or
+                                     | rewrite !(fun var => @lookupb_extendb_full flat_type _ symbolic_expr _ var _ SymbolicExprContextOk)
+                                     | setoid_rewrite in_app_iff
+                                     | break_innermost_match_step
+                                     | progress simpl in *
+                                     | discriminate
+                                     | assumption
+                                     | symmetry; assumption
+                                     | reflexivity
+                                     | progress intros
+                                     | match goal with
+                                       | [ H : ?x = Some ?a, H' : ?x = Some ?b |- _ ]
+                                         => assert (a = b) by (clear -H H'; congruence);
+                                            (subst a || subst b)
+                                       | [ H : ?x <> ?x |- _ ] => exfalso; apply H; clear
+                                       | [ H : lookupb ?t ?m ?n = Some _ |- None = @lookupb _ _ _ ?C ?t' ?m ?n ]
+                                         => let H' := fresh in
+                                            let RHS := match goal with |- _ = ?RHS => RHS end in
+                                            destruct RHS eqn:H'; [ | reflexivity ]
+                                       | [ Hm_small : forall t k, length ?m <= k -> lookupb ?m (SVar k) = None, H : lookupb ?m (SVar ?k') = Some _ |- _ ]
+                                         => rewrite Hm_small in H by omega
+                                       | [ Hm_small : forall t k, length ?m <= k -> lookupb ?m (SVar k) = None |- context[lookupb ?m (SVar ?k')] ]
+                                         => rewrite Hm_small by omega
+                                       | [ H : lookupb ?t ?m ?n = Some _, H' : lookupb ?t' ?m ?n = Some _ |- _ ]
+                                         => let H'' := fresh in
+                                            pose proof (@lookupb_unique_type _ _ _ _ SymbolicExprContextOk m n t t') as H'';
+                                            rewrite H, H' in H'';
+                                            specialize_by congruence;
+                                            (subst t || subst t')
+                                       | [ H : lookupb ?m ?s = Some ?k, H' : denote_symbolic_expr ?m _ ?s = Some ?k', Hm : forall t sv v, lookupb ?m sv = Some v -> denote_symbolic_expr ?m t sv = Some v |- _ ]
+                                         => let H'' := fresh in
+                                            pose proof (Hm _ _ _ H) as H'';
+                                            rewrite H' in H''; inversion_option;
+                                            (subst k || subst k')
+                                       | [ H : lookupb ?t ?m ?s = Some ?k, H' : denote_symbolic_expr ?m ?t' ?s = Some ?k', Hm : forall T sv v, lookupb ?m sv = Some v -> denote_symbolic_expr ?m T sv = Some v |- _ ]
+                                         => let H'' := fresh in
+                                            let H''' := fresh in
+                                            pose proof (Hm _ _ _ H) as H'';
+                                            pose proof (denote_symbolic_expr_two_types m t t' s) as H''';
+                                            rewrite H', H'' in H''';
+                                            specialize_by congruence;
+                                            (subst t || subst t')
+                                       | [ |- denote_symbolic_expr ?m ?t ?e = Some ?v ]
+                                         => lazymatch m with
+                                            | extendb ?m' _ _
+                                              => apply (fun pf1 => denote_symbolic_expr_weaken m' m pf1 t e v); [ intros ??? | ]
+                                            end
+                                       end ] ].
+        Focus 2.
+        { match goal with
+          | [ |- denote_symbolic_expr ?m ?t ?e = Some ?v ]
+            => lazymatch m with
+               | extendb ?m' _ _
+                 => apply (fun pf1 => denote_symbolic_expr_weaken m' m pf1 t e v); [ intros ??? | ]
+               end
+          end.
+        all:try solve [ repeat first [ progress subst
+                                     | progress inversion_option
+                                     | progress intros *
+                                     | progress cbn [eq_rect eq_rec eq_ind]
+                                     | solve [ eauto using interpf_flatten_binding_list, denote_symbolic_expr_flatten_binding_list ]
+                                     | progress destruct_head'_or
+                                     | rewrite !(fun var => @lookupb_extendb_full flat_type _ symbolic_expr _ var _ SymbolicExprContextOk)
+                                     | setoid_rewrite in_app_iff
+                                     | break_innermost_match_step
+                                     | progress simpl in *
+                                     | discriminate
+                                     | assumption
+                                     | symmetry; assumption
+                                     | reflexivity
+                                     | progress intros
+                                     | match goal with
+                                       | [ H : ?x = Some ?a, H' : ?x = Some ?b |- _ ]
+                                         => assert (a = b) by (clear -H H'; congruence);
+                                            (subst a || subst b)
+                                       | [ H : ?x <> ?x |- _ ] => exfalso; apply H; clear
+                                       | [ H : lookupb ?t ?m ?n = Some _ |- None = @lookupb _ _ _ ?C ?t' ?m ?n ]
+                                         => let H' := fresh in
+                                            let RHS := match goal with |- _ = ?RHS => RHS end in
+                                            destruct RHS eqn:H'; [ | reflexivity ]
+                                       | [ Hm_small : forall t k, length ?m <= k -> lookupb ?m (SVar k) = None, H : lookupb ?m (SVar ?k') = Some _ |- _ ]
+                                         => rewrite Hm_small in H by omega
+                                       | [ Hm_small : forall t k, length ?m <= k -> lookupb ?m (SVar k) = None |- context[lookupb ?m (SVar ?k')] ]
+                                         => rewrite Hm_small by omega
+                                       | [ H : lookupb ?t ?m ?n = Some _, H' : lookupb ?t' ?m ?n = Some _ |- _ ]
+                                         => let H'' := fresh in
+                                            pose proof (@lookupb_unique_type _ _ _ _ SymbolicExprContextOk m n t t') as H'';
+                                            rewrite H, H' in H'';
+                                            specialize_by congruence;
+                                            (subst t || subst t')
+                                       | [ H : lookupb ?m ?s = Some ?k, H' : denote_symbolic_expr ?m _ ?s = Some ?k', Hm : forall t sv v, lookupb ?m sv = Some v -> denote_symbolic_expr ?m t sv = Some v |- _ ]
+                                         => let H'' := fresh in
+                                            pose proof (Hm _ _ _ H) as H'';
+                                            rewrite H' in H''; inversion_option;
+                                            (subst k || subst k')
+                                       | [ H : lookupb ?t ?m ?s = Some ?k, H' : denote_symbolic_expr ?m ?t' ?s = Some ?k', Hm : forall T sv v, lookupb ?m sv = Some v -> denote_symbolic_expr ?m T sv = Some v |- _ ]
+                                         => let H'' := fresh in
+                                            let H''' := fresh in
+                                            pose proof (Hm _ _ _ H) as H'';
+                                            pose proof (denote_symbolic_expr_two_types m t t' s) as H''';
+                                            rewrite H', H'' in H''';
+                                            specialize_by congruence;
+                                            (subst t || subst t')
+                                       | [ |- denote_symbolic_expr ?m ?t ?e = Some ?v ]
+                                         => lazymatch m with
+                                            | extendb ?m' _ _
+                                              => apply (fun pf1 => denote_symbolic_expr_weaken m' m pf1 t e v); [ intros ??? | ]
+                                            end
+                                       end ] ].
+
+        repeat first [ progress subst
+                                     | progress inversion_option
+                                     | progress intros *
+                                     | progress cbn [eq_rect eq_rec eq_ind]
+                                     | solve [ eauto using interpf_flatten_binding_list, denote_symbolic_expr_flatten_binding_list ]
+                                     | progress destruct_head'_or
+                                     | rewrite !(fun var => @lookupb_extendb_full flat_type _ symbolic_expr _ var _ SymbolicExprContextOk)
+                                     | setoid_rewrite in_app_iff
+                                     | break_innermost_match_step
+                                     | progress simpl in *
+                                     | discriminate
+                                     | assumption
+                                     | symmetry; assumption
+                                     | reflexivity
+                                     | progress intros
+                                     | match goal with
+                                       | [ H : ?x = Some ?a, H' : ?x = Some ?b |- _ ]
+                                         => assert (a = b) by (clear -H H'; congruence);
+                                            (subst a || subst b)
+                                       | [ H : ?x <> ?x |- _ ] => exfalso; apply H; clear
+                                       | [ H : lookupb ?t ?m ?n = Some _ |- None = @lookupb _ _ _ ?C ?t' ?m ?n ]
+                                         => let H' := fresh in
+                                            let RHS := match goal with |- _ = ?RHS => RHS end in
+                                            destruct RHS eqn:H'; [ | reflexivity ]
+                                       | [ Hm_small : forall t k, length ?m <= k -> lookupb ?m (SVar k) = None, H : lookupb ?m (SVar ?k') = Some _ |- _ ]
+                                         => rewrite Hm_small in H by omega
+                                       | [ Hm_small : forall t k, length ?m <= k -> lookupb ?m (SVar k) = None |- context[lookupb ?m (SVar ?k')] ]
+                                         => rewrite Hm_small by omega
+                                       | [ H : lookupb ?t ?m ?n = Some _, H' : lookupb ?t' ?m ?n = Some _ |- _ ]
+                                         => let H'' := fresh in
+                                            pose proof (@lookupb_unique_type _ _ _ _ SymbolicExprContextOk m n t t') as H'';
+                                            rewrite H, H' in H'';
+                                            specialize_by congruence;
+                                            (subst t || subst t')
+                                       | [ H : lookupb ?m ?s = Some ?k, H' : denote_symbolic_expr ?m _ ?s = Some ?k', Hm : forall t sv v, lookupb ?m sv = Some v -> denote_symbolic_expr ?m t sv = Some v |- _ ]
+                                         => let H'' := fresh in
+                                            pose proof (Hm _ _ _ H) as H'';
+                                            rewrite H' in H''; inversion_option;
+                                            (subst k || subst k')
+                                       | [ H : lookupb ?t ?m ?s = Some ?k, H' : denote_symbolic_expr ?m ?t' ?s = Some ?k', Hm : forall T sv v, lookupb ?m sv = Some v -> denote_symbolic_expr ?m T sv = Some v |- _ ]
+                                         => let H'' := fresh in
+                                            let H''' := fresh in
+                                            pose proof (Hm _ _ _ H) as H'';
+                                            pose proof (denote_symbolic_expr_two_types m t t' s) as H''';
+                                            rewrite H', H'' in H''';
+                                            specialize_by congruence;
+                                            (subst t || subst t')
+                                       | [ |- denote_symbolic_expr ?m ?t ?e = Some ?v ]
+                                         => lazymatch m with
+                                            | extendb ?m' _ _
+                                              => apply (fun pf1 => denote_symbolic_expr_weaken m' m pf1 t e v); [ intros ??? | ]
+                                            end
+                                       end ].
+        Focus 2.
+        all:try solve [ repeat first [ progress subst
+                                     | progress inversion_option
+                                     | progress intros *
+                                     | progress cbn [eq_rect eq_rec eq_ind]
+                                     | solve [ eauto using interpf_flatten_binding_list, denote_symbolic_expr_flatten_binding_list ]
+                                     | progress destruct_head'_or
+                                     | rewrite !(fun var => @lookupb_extendb_full flat_type _ symbolic_expr _ var _ SymbolicExprContextOk)
+                                     | setoid_rewrite in_app_iff
+                                     | break_innermost_match_step
+                                     | progress simpl in *
+                                     | discriminate
+                                     | assumption
+                                     | symmetry; assumption
+                                     | reflexivity
+                                     | progress intros
+                                     | match goal with
+                                       | [ H : ?x = Some ?a, H' : ?x = Some ?b |- _ ]
+                                         => assert (a = b) by (clear -H H'; congruence);
+                                            (subst a || subst b)
+                                       | [ H : ?x <> ?x |- _ ] => exfalso; apply H; clear
+                                       | [ H : lookupb ?t ?m ?n = Some _ |- None = @lookupb _ _ _ ?C ?t' ?m ?n ]
+                                         => let H' := fresh in
+                                            let RHS := match goal with |- _ = ?RHS => RHS end in
+                                            destruct RHS eqn:H'; [ | reflexivity ]
+                                       | [ Hm_small : forall t k, length ?m <= k -> lookupb ?m (SVar k) = None, H : lookupb ?m (SVar ?k') = Some _ |- _ ]
+                                         => rewrite Hm_small in H by omega
+                                       | [ Hm_small : forall t k, length ?m <= k -> lookupb ?m (SVar k) = None |- context[lookupb ?m (SVar ?k')] ]
+                                         => rewrite Hm_small by omega
+                                       | [ H : lookupb ?t ?m ?n = Some _, H' : lookupb ?t' ?m ?n = Some _ |- _ ]
+                                         => let H'' := fresh in
+                                            pose proof (@lookupb_unique_type _ _ _ _ SymbolicExprContextOk m n t t') as H'';
+                                            rewrite H, H' in H'';
+                                            specialize_by congruence;
+                                            (subst t || subst t')
+                                       | [ H : lookupb ?m ?s = Some ?k, H' : denote_symbolic_expr ?m _ ?s = Some ?k', Hm : forall t sv v, lookupb ?m sv = Some v -> denote_symbolic_expr ?m t sv = Some v |- _ ]
+                                         => let H'' := fresh in
+                                            pose proof (Hm _ _ _ H) as H'';
+                                            rewrite H' in H''; inversion_option;
+                                            (subst k || subst k')
+                                       | [ H : lookupb ?t ?m ?s = Some ?k, H' : denote_symbolic_expr ?m ?t' ?s = Some ?k', Hm : forall T sv v, lookupb ?m sv = Some v -> denote_symbolic_expr ?m T sv = Some v |- _ ]
+                                         => let H'' := fresh in
+                                            let H''' := fresh in
+                                            pose proof (Hm _ _ _ H) as H'';
+                                            pose proof (denote_symbolic_expr_two_types m t t' s) as H''';
+                                            rewrite H', H'' in H''';
+                                            specialize_by congruence;
+                                            (subst t || subst t')
+                                       | [ |- denote_symbolic_expr ?m ?t ?e = Some ?v ]
+                                         => lazymatch m with
+                                            | extendb ?m' _ _
+                                              => apply (fun pf1 => denote_symbolic_expr_weaken m' m pf1 t e v); [ intros ??? | ]
+                                            end
+                                       end ]
+
+                        | repeat first [ progress cbn [denote_symbolic_expr fst snd projT1 projT2]
+                                       | setoid_rewrite length_extendb
+                                       | rewrite Nat.sub_diag
+                                       | reflexivity
+                                       | discriminate
+                                       | rewrite eq_trans_sym_inv_r
+                                       | progress simpl @nth_error
+                                       | progress unfold var_cast;
+                                         break_innermost_match
+                                       | match goal with
+                                         | [ H : context[flat_type_beq _ _ ?x ?x] |- _ ]
+                                           => setoid_rewrite (flat_type_dec_lb _ _ base_type_code_lb x x eq_refl) in H
+                                         end ] ].
+        {
+
+          repeat first [ progress subst
+                                     | progress inversion_option
+                                     | progress intros *
+                                     | progress cbn [eq_rect eq_rec eq_ind]
+                                     | solve [ eauto using interpf_flatten_binding_list, denote_symbolic_expr_flatten_binding_list ]
+                                     | progress destruct_head'_or
+                                     | rewrite !(fun var => @lookupb_extendb_full flat_type _ symbolic_expr _ var _ SymbolicExprContextOk)
+                                     | setoid_rewrite in_app_iff
+                                     | break_innermost_match_step
+                                     | progress simpl in *
+                                     | discriminate
+                                     | assumption
+                                     | symmetry; assumption
+                                     | reflexivity
+                                     | progress intros
+                                     | match goal with
+                                       | [ H : ?x = Some ?a, H' : ?x = Some ?b |- _ ]
+                                         => assert (a = b) by (clear -H H'; congruence);
+                                            (subst a || subst b)
+                                       | [ H : ?x <> ?x |- _ ] => exfalso; apply H; clear
+                                       | [ H : lookupb ?t ?m ?n = Some _ |- None = @lookupb _ _ _ ?C ?t' ?m ?n ]
+                                         => let H' := fresh in
+                                            let RHS := match goal with |- _ = ?RHS => RHS end in
+                                            destruct RHS eqn:H'; [ | reflexivity ]
+                                       | [ Hm_small : forall t k, length ?m <= k -> lookupb ?m (SVar k) = None, H : lookupb ?m (SVar ?k') = Some _ |- _ ]
+                                         => rewrite Hm_small in H by omega
+                                       | [ Hm_small : forall t k, length ?m <= k -> lookupb ?m (SVar k) = None |- context[lookupb ?m (SVar ?k')] ]
+                                         => rewrite Hm_small by omega
+                                       | [ H : lookupb ?t ?m ?n = Some _, H' : lookupb ?t' ?m ?n = Some _ |- _ ]
+                                         => let H'' := fresh in
+                                            pose proof (@lookupb_unique_type _ _ _ _ SymbolicExprContextOk m n t t') as H'';
+                                            rewrite H, H' in H'';
+                                            specialize_by congruence;
+                                            (subst t || subst t')
+                                       | [ H : lookupb ?m ?s = Some ?k, H' : denote_symbolic_expr ?m _ ?s = Some ?k', Hm : forall t sv v, lookupb ?m sv = Some v -> denote_symbolic_expr ?m t sv = Some v |- _ ]
+                                         => let H'' := fresh in
+                                            pose proof (Hm _ _ _ H) as H'';
+                                            rewrite H' in H''; inversion_option;
+                                            (subst k || subst k')
+                                       | [ H : lookupb ?t ?m ?s = Some ?k, H' : denote_symbolic_expr ?m ?t' ?s = Some ?k', Hm : forall T sv v, lookupb ?m sv = Some v -> denote_symbolic_expr ?m T sv = Some v |- _ ]
+                                         => let H'' := fresh in
+                                            let H''' := fresh in
+                                            pose proof (Hm _ _ _ H) as H'';
+                                            pose proof (denote_symbolic_expr_two_types m t t' s) as H''';
+                                            rewrite H', H'' in H''';
+                                            specialize_by congruence;
+                                            (subst t || subst t')
+                                       end ].
+        all:try solve [ repeat first [ progress subst
+                                     | progress inversion_option
+                                     | progress intros *
+                                     | progress cbn [eq_rect eq_rec eq_ind]
+                                     | solve [ eauto using interpf_flatten_binding_list, denote_symbolic_expr_flatten_binding_list ]
+                                     | progress destruct_head'_or
+                                     | rewrite !(fun var => @lookupb_extendb_full flat_type _ symbolic_expr _ var _ SymbolicExprContextOk)
+                                     | setoid_rewrite in_app_iff
+                                     | break_innermost_match_step
+                                     | progress simpl in *
+                                     | discriminate
+                                     | assumption
+                                     | symmetry; assumption
+                                     | reflexivity
+                                     | progress intros
+                                     | match goal with
+                                       | [ H : ?x = Some ?a, H' : ?x = Some ?b |- _ ]
+                                         => assert (a = b) by (clear -H H'; congruence);
+                                            (subst a || subst b)
+                                       | [ H : ?x <> ?x |- _ ] => exfalso; apply H; clear
+                                       | [ H : lookupb ?t ?m ?n = Some _ |- None = @lookupb _ _ _ ?C ?t' ?m ?n ]
+                                         => let H' := fresh in
+                                            let RHS := match goal with |- _ = ?RHS => RHS end in
+                                            destruct RHS eqn:H'; [ | reflexivity ]
+                                       | [ Hm_small : forall t k, length ?m <= k -> lookupb ?m (SVar k) = None, H : lookupb ?m (SVar ?k') = Some _ |- _ ]
+                                         => rewrite Hm_small in H by omega
+                                       | [ Hm_small : forall t k, length ?m <= k -> lookupb ?m (SVar k) = None |- context[lookupb ?m (SVar ?k')] ]
+                                         => rewrite Hm_small by omega
+                                       | [ H : lookupb ?t ?m ?n = Some _, H' : lookupb ?t' ?m ?n = Some _ |- _ ]
+                                         => let H'' := fresh in
+                                            pose proof (@lookupb_unique_type _ _ _ _ SymbolicExprContextOk m n t t') as H'';
+                                            rewrite H, H' in H'';
+                                            specialize_by congruence;
+                                            (subst t || subst t')
+                                       | [ H : lookupb ?m ?s = Some ?k, H' : denote_symbolic_expr ?m _ ?s = Some ?k', Hm : forall t sv v, lookupb ?m sv = Some v -> denote_symbolic_expr ?m t sv = Some v |- _ ]
+                                         => let H'' := fresh in
+                                            pose proof (Hm _ _ _ H) as H'';
+                                            rewrite H' in H''; inversion_option;
+                                            (subst k || subst k')
+                                       | [ H : lookupb ?t ?m ?s = Some ?k, H' : denote_symbolic_expr ?m ?t' ?s = Some ?k', Hm : forall T sv v, lookupb ?m sv = Some v -> denote_symbolic_expr ?m T sv = Some v |- _ ]
+                                         => let H'' := fresh in
+                                            let H''' := fresh in
+                                            pose proof (Hm _ _ _ H) as H'';
+                                            pose proof (denote_symbolic_expr_two_types m t t' s) as H''';
+                                            rewrite H', H'' in H''';
+                                            specialize_by congruence;
+                                            (subst t || subst t')
+                                       | [ |- denote_symbolic_expr ?m ?t ?e = Some ?v ]
+                                         => lazymatch m with
+                                            | extendb ?m' _ _
+                                              => apply (fun pf1 => denote_symbolic_expr_weaken m' m pf1 t e v); [ intros ??? | ]
+                                            end
+                                       end ]
+
+                        | repeat first [ progress cbn [denote_symbolic_expr fst snd projT1 projT2]
+                                       | setoid_rewrite length_extendb
+                                       | rewrite Nat.sub_diag
+                                       | reflexivity
+                                       | discriminate
+                                       | rewrite eq_trans_sym_inv_r
+                                       | progress simpl @nth_error
+                                       | progress unfold var_cast;
+                                         break_innermost_match
+                                       | match goal with
+                                         | [ H : context[flat_type_beq _ _ ?x ?x] |- _ ]
+                                           => setoid_rewrite (flat_type_dec_lb _ _ base_type_code_lb x x eq_refl) in H
+                                         end ] ].
+
+                                       | [ |- denote_symbolic_expr ?m ?t ?e = Some ?v ]
+                                         => lazymatch m with
+                                            | extendb ?m' _ _
+                                              => apply (fun pf1 => denote_symbolic_expr_weaken m' m pf1 t e v); [ intros ??? | ]
+                                            end
+                                       end ]
+                      .
+        2:try solve [ repeat first [ progress subst
+                                     | progress inversion_option
+                                     | progress intros *
+                                     | progress cbn [eq_rect eq_rec eq_ind]
+                                     | solve [ eauto using interpf_flatten_binding_list, denote_symbolic_expr_flatten_binding_list ]
+                                     | progress destruct_head'_or
+                                     | rewrite !(fun var => @lookupb_extendb_full flat_type _ symbolic_expr _ var _ SymbolicExprContextOk)
+                                     | setoid_rewrite in_app_iff
+                                     | break_innermost_match_step
+                                     | progress simpl in *
+                                     | discriminate
+                                     | assumption
+                                     | symmetry; assumption
+                                     | reflexivity
+                                     | progress intros
+                                     | match goal with
+                                       | [ H : ?x = Some ?a, H' : ?x = Some ?b |- _ ]
+                                         => assert (a = b) by (clear -H H'; congruence);
+                                            (subst a || subst b)
+                                       | [ H : ?x <> ?x |- _ ] => exfalso; apply H; clear
+                                       | [ H : lookupb ?t ?m ?n = Some _ |- None = @lookupb _ _ _ ?C ?t' ?m ?n ]
+                                         => let H' := fresh in
+                                            let RHS := match goal with |- _ = ?RHS => RHS end in
+                                            destruct RHS eqn:H'; [ | reflexivity ]
+                                       | [ Hm_small : forall t k, length ?m <= k -> lookupb ?m (SVar k) = None, H : lookupb ?m (SVar ?k') = Some _ |- _ ]
+                                         => rewrite Hm_small in H by omega
+                                       | [ Hm_small : forall t k, length ?m <= k -> lookupb ?m (SVar k) = None |- context[lookupb ?m (SVar ?k')] ]
+                                         => rewrite Hm_small by omega
+                                       | [ H : lookupb ?t ?m ?n = Some _, H' : lookupb ?t' ?m ?n = Some _ |- _ ]
+                                         => let H'' := fresh in
+                                            pose proof (@lookupb_unique_type _ _ _ _ SymbolicExprContextOk m n t t') as H'';
+                                            rewrite H, H' in H'';
+                                            specialize_by congruence;
+                                            (subst t || subst t')
+                                       | [ H : lookupb ?m ?s = Some ?k, H' : denote_symbolic_expr ?m _ ?s = Some ?k', Hm : forall t sv v, lookupb ?m sv = Some v -> denote_symbolic_expr ?m t sv = Some v |- _ ]
+                                         => let H'' := fresh in
+                                            pose proof (Hm _ _ _ H) as H'';
+                                            rewrite H' in H''; inversion_option;
+                                            (subst k || subst k')
+                                       | [ H : lookupb ?t ?m ?s = Some ?k, H' : denote_symbolic_expr ?m ?t' ?s = Some ?k', Hm : forall T sv v, lookupb ?m sv = Some v -> denote_symbolic_expr ?m T sv = Some v |- _ ]
+                                         => let H'' := fresh in
+                                            let H''' := fresh in
+                                            pose proof (Hm _ _ _ H) as H'';
+                                            pose proof (denote_symbolic_expr_two_types m t t' s) as H''';
+                                            rewrite H', H'' in H''';
+                                            specialize_by congruence;
+                                            (subst t || subst t')
+                                       | [ |- denote_symbolic_expr ?m ?t ?e = Some ?v ]
+                                         => lazymatch m with
+                                            | extendb ?m' _ _
+                                              => apply (fun pf1 => denote_symbolic_expr_weaken m' m pf1 t e v); [ intros ??? | ]
+                                            end
+                                       end ] ].
+        Focus 2.
+        { repeat first [ progress subst
+                                     | progress inversion_option
+                                     | progress intros *
+                                     | progress cbn [eq_rect eq_rec eq_ind]
+                                     | solve [ eauto using interpf_flatten_binding_list, denote_symbolic_expr_flatten_binding_list ]
+                                     | progress destruct_head'_or
+                                     | rewrite !(fun var => @lookupb_extendb_full flat_type _ symbolic_expr _ var _ SymbolicExprContextOk)
+                                     | setoid_rewrite in_app_iff
+                                     | break_innermost_match_step
+                                     | progress simpl in *
+                                     | discriminate
+                                     | assumption
+                                     | symmetry; assumption
+                                     | reflexivity
+                                     | progress intros
+                                     | match goal with
+                                       | [ H : ?x = Some ?a, H' : ?x = Some ?b |- _ ]
+                                         => assert (a = b) by (clear -H H'; congruence);
+                                            (subst a || subst b)
+                                       | [ H : ?x <> ?x |- _ ] => exfalso; apply H; clear
+                                       | [ H : lookupb ?t ?m ?n = Some _ |- None = @lookupb _ _ _ ?C ?t' ?m ?n ]
+                                         => let H' := fresh in
+                                            let RHS := match goal with |- _ = ?RHS => RHS end in
+                                            destruct RHS eqn:H'; [ | reflexivity ]
+                                       | [ Hm_small : forall t k, length ?m <= k -> lookupb ?m (SVar k) = None, H : lookupb ?m (SVar ?k') = Some _ |- _ ]
+                                         => rewrite Hm_small in H by omega
+                                       | [ Hm_small : forall t k, length ?m <= k -> lookupb ?m (SVar k) = None |- context[lookupb ?m (SVar ?k')] ]
+                                         => rewrite Hm_small by omega
+                                       | [ H : lookupb ?t ?m ?n = Some _, H' : lookupb ?t' ?m ?n = Some _ |- _ ]
+                                         => let H'' := fresh in
+                                            pose proof (@lookupb_unique_type _ _ _ _ SymbolicExprContextOk m n t t') as H'';
+                                            rewrite H, H' in H'';
+                                            specialize_by congruence;
+                                            (subst t || subst t')
+                                       | [ H : lookupb ?m ?s = Some ?k, H' : denote_symbolic_expr ?m _ ?s = Some ?k', Hm : forall t sv v, lookupb ?m sv = Some v -> denote_symbolic_expr ?m t sv = Some v |- _ ]
+                                         => let H'' := fresh in
+                                            pose proof (Hm _ _ _ H) as H'';
+                                            rewrite H' in H''; inversion_option;
+                                            (subst k || subst k')
+                                       | [ H : lookupb ?t ?m ?s = Some ?k, H' : denote_symbolic_expr ?m ?t' ?s = Some ?k', Hm : forall T sv v, lookupb ?m sv = Some v -> denote_symbolic_expr ?m T sv = Some v |- _ ]
+                                         => let H'' := fresh in
+                                            let H''' := fresh in
+                                            pose proof (Hm _ _ _ H) as H'';
+                                            pose proof (denote_symbolic_expr_two_types m t t' s) as H''';
+                                            rewrite H', H'' in H''';
+                                            specialize_by congruence;
+                                            (subst t || subst t')
+                                       | [ |- denote_symbolic_expr ?m ?t ?e = Some ?v ]
+                                         => lazymatch m with
+                                            | extendb ?m' _ _
+                                              => apply (fun pf1 => denote_symbolic_expr_weaken m' m pf1 t e v); [ intros ??? | ]
+                                            end
+                                       end ].
+
+
+        { repeat first [ progress subst
+                                     | progress inversion_option
+                                     | progress intros *
+                                     | progress cbn [eq_rect eq_rec eq_ind]
+                                     | solve [ eauto using interpf_flatten_binding_list, denote_symbolic_expr_flatten_binding_list ]
+                                     | progress destruct_head'_or
+                                     | rewrite !(fun var => @lookupb_extendb_full flat_type _ symbolic_expr _ var _ SymbolicExprContextOk)
+                                     | setoid_rewrite in_app_iff
+                                     | break_innermost_match_step
+                                     | progress simpl in *
+                                     | discriminate
+                                     | assumption
+                                     | symmetry; assumption
+                                     | reflexivity
+                                     | progress intros
+                                     | match goal with
+                                       | [ H : ?x = Some ?a, H' : ?x = Some ?b |- _ ]
+                                         => assert (a = b) by (clear -H H'; congruence);
+                                            (subst a || subst b)
+                                       | [ H : ?x <> ?x |- _ ] => exfalso; apply H; clear
+                                       | [ H : lookupb ?t ?m ?n = Some _ |- None = @lookupb _ _ _ ?C ?t' ?m ?n ]
+                                         => let H' := fresh in
+                                            let RHS := match goal with |- _ = ?RHS => RHS end in
+                                            destruct RHS eqn:H'; [ | reflexivity ]
+                                       | [ Hm_small : forall t k, length ?m <= k -> lookupb ?m (SVar k) = None, H : lookupb ?m (SVar ?k') = Some _ |- _ ]
+                                         => rewrite Hm_small in H by omega
+                                       | [ Hm_small : forall t k, length ?m <= k -> lookupb ?m (SVar k) = None |- context[lookupb ?m (SVar ?k')] ]
+                                         => rewrite Hm_small by omega
+                                       | [ H : lookupb ?t ?m ?n = Some _, H' : lookupb ?t' ?m ?n = Some _ |- _ ]
+                                         => let H'' := fresh in
+                                            pose proof (@lookupb_unique_type _ _ _ _ SymbolicExprContextOk m n t t') as H'';
+                                            rewrite H, H' in H'';
+                                            specialize_by congruence;
+                                            (subst t || subst t')
+                                       | [ H : lookupb ?m ?s = Some ?k, H' : denote_symbolic_expr ?m _ ?s = Some ?k', Hm : forall t sv v, lookupb ?m sv = Some v -> denote_symbolic_expr ?m t sv = Some v |- _ ]
+                                         => let H'' := fresh in
+                                            pose proof (Hm _ _ _ H) as H'';
+                                            rewrite H' in H''; inversion_option;
+                                            (subst k || subst k')
+                                       | [ H : lookupb ?t ?m ?s = Some ?k, H' : denote_symbolic_expr ?m ?t' ?s = Some ?k', Hm : forall T sv v, lookupb ?m sv = Some v -> denote_symbolic_expr ?m T sv = Some v |- _ ]
+                                         => let H'' := fresh in
+                                            let H''' := fresh in
+                                            pose proof (Hm _ _ _ H) as H'';
+                                            pose proof (denote_symbolic_expr_two_types m t t' s) as H''';
+                                            rewrite H', H'' in H''';
+                                            specialize_by congruence;
+                                            (subst t || subst t')
+                                       end ].
+          admit. }
+        { repeat first [ progress subst
+                       | progress inversion_option
+                       | progress intros *
+                       | progress cbn [eq_rect eq_rec eq_ind]
+                       | solve [ eauto using interpf_flatten_binding_list, denote_symbolic_expr_flatten_binding_list ]
+                       | progress destruct_head'_or
+                       | rewrite !(fun var => @lookupb_extendb_full flat_type _ symbolic_expr _ var _ SymbolicExprContextOk)
+                       | setoid_rewrite in_app_iff
+                       | break_innermost_match_step
+                       | progress simpl in *
+                       | discriminate
+                       | assumption
+                       | symmetry; assumption
+                       | reflexivity
+                       | progress intros
+                       | match goal with
+                         | [ H : ?x = Some ?a, H' : ?x = Some ?b |- _ ]
+                           => assert (a = b) by (clear -H H'; congruence);
+                              (subst a || subst b)
+                         | [ H : ?x <> ?x |- _ ] => exfalso; apply H; clear
+                         | [ H : lookupb ?t ?m ?n = Some _ |- None = @lookupb _ _ _ ?C ?t' ?m ?n ]
+                           => let H' := fresh in
+                              let RHS := match goal with |- _ = ?RHS => RHS end in
+                              destruct RHS eqn:H'; [ | reflexivity ]
+                         | [ Hm_small : forall t k, length ?m <= k -> lookupb ?m (SVar k) = None, H : lookupb ?m (SVar ?k') = Some _ |- _ ]
+                           => rewrite Hm_small in H by omega
+                         | [ Hm_small : forall t k, length ?m <= k -> lookupb ?m (SVar k) = None |- context[lookupb ?m (SVar ?k')] ]
+                           => rewrite Hm_small by omega
+                         | [ H : lookupb ?t ?m ?n = Some _, H' : lookupb ?t' ?m ?n = Some _ |- _ ]
+                           => let H'' := fresh in
+                              pose proof (@lookupb_unique_type _ _ _ _ SymbolicExprContextOk m n t t') as H'';
+                              rewrite H, H' in H'';
+                              specialize_by congruence;
+                              (subst t || subst t')
+                         | [ H : lookupb ?m ?s = Some ?k, H' : denote_symbolic_expr ?m _ ?s = Some ?k', Hm : forall t sv v, lookupb ?m sv = Some v -> denote_symbolic_expr ?m t sv = Some v |- _ ]
+                           => let H'' := fresh in
+                              pose proof (Hm _ _ _ H) as H'';
+                              rewrite H' in H''; inversion_option;
+                              (subst k || subst k')
+                         | [ H : lookupb ?t ?m ?s = Some ?k, H' : denote_symbolic_expr ?m ?t' ?s = Some ?k', Hm : forall T sv v, lookupb ?m sv = Some v -> denote_symbolic_expr ?m T sv = Some v |- _ ]
+                           => let H'' := fresh in
+                              let H''' := fresh in
+                              pose proof (Hm _ _ _ H) as H'';
+                              pose proof (denote_symbolic_expr_two_types m t t' s) as H''';
+                              rewrite H', H'' in H''';
+                              specialize_by congruence;
+                              (subst t || subst t')
+                         end ].
+          { eapply denote_symbolic_expr_flatten_binding_list.
+            all:repeat first [ progress subst
+                           | progress inversion_option
+                           | progress intros *
+                           | progress cbn [eq_rect eq_rec eq_ind]
+                           | solve [ eauto using interpf_flatten_binding_list, denote_symbolic_expr_flatten_binding_list ]
+                           | progress destruct_head'_or
+                           | rewrite !(fun var => @lookupb_extendb_full flat_type _ symbolic_expr _ var _ SymbolicExprContextOk)
+                           | setoid_rewrite in_app_iff
+                           | break_innermost_match_step
+                           | intros; progress inversion_option ].
+          all:try solve [ repeat first [ progress subst
+                                       | progress inversion_option
+                                       | progress intros *
+                                       | progress cbn [eq_rect eq_rec eq_ind]
+                                       | solve [ eauto using interpf_flatten_binding_list, denote_symbolic_expr_flatten_binding_list ]
+                                       | progress destruct_head'_or
+                                       | rewrite !(fun var => @lookupb_extendb_full flat_type _ symbolic_expr _ var _ SymbolicExprContextOk)
+                                       | setoid_rewrite in_app_iff
+                                       | break_innermost_match_step
+                                       | progress simpl in *
+                                       | discriminate
+                                       | assumption
+                                       | symmetry; assumption
+                                       | reflexivity
+                                       | progress intros
+                                       | match goal with
+                                         | [ H : ?x = Some ?a, H' : ?x = Some ?b |- _ ]
+                                           => assert (a = b) by (clear -H H'; congruence);
+                                              (subst a || subst b)
+                                         | [ H : ?x <> ?x |- _ ] => exfalso; apply H; clear
+                                         | [ H : lookupb ?t ?m ?n = Some _ |- None = @lookupb _ _ _ ?C ?t' ?m ?n ]
+                                           => let H' := fresh in
+                                              let RHS := match goal with |- _ = ?RHS => RHS end in
+                                              destruct RHS eqn:H'; [ | reflexivity ]
+                                         | [ Hm_small : forall t k, length ?m <= k -> lookupb ?m (SVar k) = None, H : lookupb ?m (SVar ?k') = Some _ |- _ ]
+                                           => rewrite Hm_small in H by omega
+                                         | [ H : lookupb ?t ?m ?n = Some _, H' : lookupb ?t' ?m ?n = Some _ |- _ ]
+                                           => let H'' := fresh in
+                                              pose proof (@lookupb_unique_type _ _ _ _ SymbolicExprContextOk m n t t') as H'';
+                                              rewrite H, H' in H'';
+                                              specialize_by congruence;
+                                              (subst t || subst t')
+                                         | [ H : lookupb ?m ?s = Some ?k, H' : denote_symbolic_expr ?m _ ?s = Some ?k', Hm : forall t sv v, lookupb ?m sv = Some v -> denote_symbolic_expr ?m t sv = Some v |- _ ]
+                                           => let H'' := fresh in
+                                              pose proof (Hm _ _ _ H) as H'';
+                                              rewrite H' in H''; inversion_option;
+                                              (subst k || subst k')
+                                         | [ H : lookupb ?t ?m ?s = Some ?k, H' : denote_symbolic_expr ?m ?t' ?s = Some ?k', Hm : forall T sv v, lookupb ?m sv = Some v -> denote_symbolic_expr ?m T sv = Some v |- _ ]
+                                           => let H'' := fresh in
+                                              let H''' := fresh in
+                                              pose proof (Hm _ _ _ H) as H'';
+                                              pose proof (denote_symbolic_expr_two_types m t t' s) as H''';
+                                              rewrite H', H'' in H''';
+                                              specialize_by congruence;
+                                              (subst t || subst t')
+                                         | [ |- denote_symbolic_expr ?m ?t ?e = Some ?v ]
+                                           => lazymatch m with
+                                              | extendb ?m' _ _
+                                                => apply (fun pf1 => denote_symbolic_expr_weaken m' m pf1 t e v); [ intros ??? | ]
+                                              end
+                                         end ]
+                        | repeat first [ progress cbn [denote_symbolic_expr fst snd projT1 projT2]
+                                       | setoid_rewrite length_extendb
+                                       | rewrite Nat.sub_diag
+                                       | reflexivity
+                                       | discriminate
+                                       | rewrite eq_trans_sym_inv_r
+                                       | progress simpl @nth_error
+                                       | progress unfold var_cast;
+                                         break_innermost_match
+                                       | match goal with
+                                         | [ H : context[flat_type_beq _ _ ?x ?x] |- _ ]
+                                           => setoid_rewrite (flat_type_dec_lb _ _ base_type_code_lb x x eq_refl) in H
+                                         end ] ]. }
+          all:try solve [ repeat first [ progress subst
+                                       | progress inversion_option
+                                       | progress intros *
+                                       | progress cbn [eq_rect eq_rec eq_ind]
+                                       | solve [ eauto using interpf_flatten_binding_list, denote_symbolic_expr_flatten_binding_list ]
+                                       | progress destruct_head'_or
+                                       | rewrite !(fun var => @lookupb_extendb_full flat_type _ symbolic_expr _ var _ SymbolicExprContextOk)
+                                       | setoid_rewrite in_app_iff
+                                       | break_innermost_match_step
+                                       | progress simpl in *
+                                       | discriminate
+                                       | assumption
+                                       | symmetry; assumption
+                                       | reflexivity
+                                       | progress intros
+                                       | match goal with
+                                         | [ H : ?x = Some ?a, H' : ?x = Some ?b |- _ ]
+                                           => assert (a = b) by (clear -H H'; congruence);
+                                              (subst a || subst b)
+                                         | [ H : ?x <> ?x |- _ ] => exfalso; apply H; clear
+                                         | [ H : lookupb ?t ?m ?n = Some _ |- None = @lookupb _ _ _ ?C ?t' ?m ?n ]
+                                           => let H' := fresh in
+                                              let RHS := match goal with |- _ = ?RHS => RHS end in
+                                              destruct RHS eqn:H'; [ | reflexivity ]
+                                         | [ Hm_small : forall t k, length ?m <= k -> lookupb ?m (SVar k) = None, H : lookupb ?m (SVar ?k') = Some _ |- _ ]
+                                           => rewrite Hm_small in H by omega
+                                         | [ H : lookupb ?t ?m ?n = Some _, H' : lookupb ?t' ?m ?n = Some _ |- _ ]
+                                           => let H'' := fresh in
+                                              pose proof (@lookupb_unique_type _ _ _ _ SymbolicExprContextOk m n t t') as H'';
+                                              rewrite H, H' in H'';
+                                              specialize_by congruence;
+                                              (subst t || subst t')
+                                         | [ H : lookupb ?m ?s = Some ?k, H' : denote_symbolic_expr ?m _ ?s = Some ?k', Hm : forall t sv v, lookupb ?m sv = Some v -> denote_symbolic_expr ?m t sv = Some v |- _ ]
+                                           => let H'' := fresh in
+                                              pose proof (Hm _ _ _ H) as H'';
+                                              rewrite H' in H''; inversion_option;
+                                              (subst k || subst k')
+                                         | [ H : lookupb ?t ?m ?s = Some ?k, H' : denote_symbolic_expr ?m ?t' ?s = Some ?k', Hm : forall T sv v, lookupb ?m sv = Some v -> denote_symbolic_expr ?m T sv = Some v |- _ ]
+                                           => let H'' := fresh in
+                                              let H''' := fresh in
+                                              pose proof (Hm _ _ _ H) as H'';
+                                              pose proof (denote_symbolic_expr_two_types m t t' s) as H''';
+                                              rewrite H', H'' in H''';
+                                              specialize_by congruence;
+                                              (subst t || subst t')
+                                         | [ |- denote_symbolic_expr ?m ?t ?e = Some ?v ]
+                                           => lazymatch m with
+                                              | extendb ?m' _ _
+                                                => apply (fun pf1 => denote_symbolic_expr_weaken m' m pf1 t e v); [ intros ??? | ]
+                                              end
+                                         end ]
+                        | repeat first [ progress cbn [denote_symbolic_expr fst snd projT1 projT2]
+                                       | setoid_rewrite length_extendb
+                                       | rewrite Nat.sub_diag
+                                       | reflexivity
+                                       | discriminate
+                                       | rewrite eq_trans_sym_inv_r
+                                       | progress simpl @nth_error
+                                       | progress unfold var_cast;
+                                         break_innermost_match
+                                       | match goal with
+                                         | [ H : context[flat_type_beq _ _ ?x ?x] |- _ ]
+                                           => setoid_rewrite (flat_type_dec_lb _ _ base_type_code_lb x x eq_refl) in H
+                                         end ] ]. }
+        all:repeat setoid_rewrite length_extendb.
+        all:repeat setoid_rewrite in_app_iff.
+        all:intros *.
+        all:rewrite ?(fun var => @lookupb_extendb_full flat_type _ symbolic_expr _ var _ SymbolicExprContextOk).
+        all:break_innermost_match; subst.
+        all:cbn [eq_rect eq_rec eq_ind]; inversion_option.
+        all:try (intro; progress inversion_option).
+        all:subst.
+        all:try solve [ repeat first [ progress subst
+                                       | progress inversion_option
+                                       | progress intros *
+                                       | progress cbn [eq_rect eq_rec eq_ind]
+                                       | solve [ eauto using interpf_flatten_binding_list, denote_symbolic_expr_flatten_binding_list ]
+                                       | progress destruct_head'_or
+                                       | rewrite !(fun var => @lookupb_extendb_full flat_type _ symbolic_expr _ var _ SymbolicExprContextOk)
+                                       | setoid_rewrite in_app_iff
+                                       | break_innermost_match_step
+                                       | progress simpl in *
+                                       | discriminate
+                                       | assumption
+                                       | symmetry; assumption
+                                       | reflexivity
+                                       | progress intros
+                                       | match goal with
+                                         | [ H : ?x = Some ?a, H' : ?x = Some ?b |- _ ]
+                                           => assert (a = b) by (clear -H H'; congruence);
+                                              (subst a || subst b)
+                                         | [ H : ?x <> ?x |- _ ] => exfalso; apply H; clear
+                                         | [ H : lookupb ?t ?m ?n = Some _ |- None = @lookupb _ _ _ ?C ?t' ?m ?n ]
+                                           => let H' := fresh in
+                                              let RHS := match goal with |- _ = ?RHS => RHS end in
+                                              destruct RHS eqn:H'; [ | reflexivity ]
+                                         | [ Hm_small : forall t k, length ?m <= k -> lookupb ?m (SVar k) = None, H : lookupb ?m (SVar ?k') = Some _ |- _ ]
+                                           => rewrite Hm_small in H by omega
+                                         | [ H : lookupb ?t ?m ?n = Some _, H' : lookupb ?t' ?m ?n = Some _ |- _ ]
+                                           => let H'' := fresh in
+                                              pose proof (@lookupb_unique_type _ _ _ _ SymbolicExprContextOk m n t t') as H'';
+                                              rewrite H, H' in H'';
+                                              specialize_by congruence;
+                                              (subst t || subst t')
+                                         | [ H : lookupb ?m ?s = Some ?k, H' : denote_symbolic_expr ?m _ ?s = Some ?k', Hm : forall t sv v, lookupb ?m sv = Some v -> denote_symbolic_expr ?m t sv = Some v |- _ ]
+                                           => let H'' := fresh in
+                                              pose proof (Hm _ _ _ H) as H'';
+                                              rewrite H' in H''; inversion_option;
+                                              (subst k || subst k')
+                                         | [ H : lookupb ?t ?m ?s = Some ?k, H' : denote_symbolic_expr ?m ?t' ?s = Some ?k', Hm : forall T sv v, lookupb ?m sv = Some v -> denote_symbolic_expr ?m T sv = Some v |- _ ]
+                                           => let H'' := fresh in
+                                              let H''' := fresh in
+                                              pose proof (Hm _ _ _ H) as H'';
+                                              pose proof (denote_symbolic_expr_two_types m t t' s) as H''';
+                                              rewrite H', H'' in H''';
+                                              specialize_by congruence;
+                                              (subst t || subst t')
+                                         | [ |- denote_symbolic_expr ?m ?t ?e = Some ?v ]
+                                           => lazymatch m with
+                                              | extendb ?m' _ _
+                                                => apply (fun pf1 => denote_symbolic_expr_weaken m' m pf1 t e v); [ intros ??? | ]
+                                              end
+                                         end ]
+                        | repeat first [ progress cbn [denote_symbolic_expr fst snd projT1 projT2]
+                                       | setoid_rewrite length_extendb
+                                       | rewrite Nat.sub_diag
+                                       | reflexivity
+                                       | discriminate
+                                       | rewrite eq_trans_sym_inv_r
+                                       | progress simpl @nth_error
+                                       | progress unfold var_cast;
+                                         break_innermost_match
+                                       | match goal with
+                                         | [ H : context[flat_type_beq _ _ ?x ?x] |- _ ]
+                                           => setoid_rewrite (flat_type_dec_lb _ _ base_type_code_lb x x eq_refl) in H
+                                         end ] ].
+        all:repeat match goal with
+                   | [ H : SVar _ = SVar _ |- _ ] => inversion H; clear H
+                   end.
+        all:subst.
+        all:try omega.
+        all: try (intros; apply Hm_small; omega).
+        all:destruct_head'_or.
+        all:try (intro; progress destruct_head'_or).
+        all:try solve [ repeat first [ progress subst
+                                       | progress inversion_option
+                                       | progress intros *
+                                       | progress cbn [eq_rect eq_rec eq_ind]
+                                       | solve [ eauto using interpf_flatten_binding_list, denote_symbolic_expr_flatten_binding_list ]
+                                       | progress destruct_head'_or
+                                       | rewrite !(fun var => @lookupb_extendb_full flat_type _ symbolic_expr _ var _ SymbolicExprContextOk)
+                                       | setoid_rewrite in_app_iff
+                                       | break_innermost_match_step
+                                       | progress simpl in *
+                                       | discriminate
+                                       | assumption
+                                       | symmetry; assumption
+                                       | reflexivity
+                                       | progress intros
+                                       | match goal with
+                                         | [ H : ?x = Some ?a, H' : ?x = Some ?b |- _ ]
+                                           => assert (a = b) by (clear -H H'; congruence);
+                                              (subst a || subst b)
+                                         | [ H : ?x <> ?x |- _ ] => exfalso; apply H; clear
+                                         | [ H : lookupb ?t ?m ?n = Some _ |- None = @lookupb _ _ _ ?C ?t' ?m ?n ]
+                                           => let H' := fresh in
+                                              let RHS := match goal with |- _ = ?RHS => RHS end in
+                                              destruct RHS eqn:H'; [ | reflexivity ]
+                                         | [ Hm_small : forall t k, length ?m <= k -> lookupb ?m (SVar k) = None, H : lookupb ?m (SVar ?k') = Some _ |- _ ]
+                                           => rewrite Hm_small in H by omega
+                                         | [ H : lookupb ?t ?m ?n = Some _, H' : lookupb ?t' ?m ?n = Some _ |- _ ]
+                                           => let H'' := fresh in
+                                              pose proof (@lookupb_unique_type _ _ _ _ SymbolicExprContextOk m n t t') as H'';
+                                              rewrite H, H' in H'';
+                                              specialize_by congruence;
+                                              (subst t || subst t')
+                                         | [ H : lookupb ?m ?s = Some ?k, H' : denote_symbolic_expr ?m _ ?s = Some ?k', Hm : forall t sv v, lookupb ?m sv = Some v -> denote_symbolic_expr ?m t sv = Some v |- _ ]
+                                           => let H'' := fresh in
+                                              pose proof (Hm _ _ _ H) as H'';
+                                              rewrite H' in H''; inversion_option;
+                                              (subst k || subst k')
+                                         | [ H : lookupb ?t ?m ?s = Some ?k, H' : denote_symbolic_expr ?m ?t' ?s = Some ?k', Hm : forall T sv v, lookupb ?m sv = Some v -> denote_symbolic_expr ?m T sv = Some v |- _ ]
+                                           => let H'' := fresh in
+                                              let H''' := fresh in
+                                              pose proof (Hm _ _ _ H) as H'';
+                                              pose proof (denote_symbolic_expr_two_types m t t' s) as H''';
+                                              rewrite H', H'' in H''';
+                                              specialize_by congruence;
+                                              (subst t || subst t')
+                                         | [ |- denote_symbolic_expr ?m ?t ?e = Some ?v ]
+                                           => lazymatch m with
+                                              | extendb ?m' _ _
+                                                => apply (fun pf1 => denote_symbolic_expr_weaken m' m pf1 t e v); [ intros ??? | ]
+                                              end
+                                         end ]
+                        | repeat first [ progress cbn [denote_symbolic_expr fst snd projT1 projT2]
+                                       | setoid_rewrite length_extendb
+                                       | rewrite Nat.sub_diag
+                                       | reflexivity
+                                       | discriminate
+                                       | rewrite eq_trans_sym_inv_r
+                                       | progress simpl @nth_error
+                                       | progress unfold var_cast;
+                                         break_innermost_match
+                                       | match goal with
+                                         | [ H : context[flat_type_beq _ _ ?x ?x] |- _ ]
+                                           => setoid_rewrite (flat_type_dec_lb _ _ base_type_code_lb x x eq_refl) in H
+                                         end ] ].
+        all:try lazymatch goal with
+                | [ H : norm_symbolize_exprf _ = Some _ |- _ ]
+                  => let H' := fresh in
+                     refine (let H' := denote_symbolic_expr_norm_symbolize_exprf H _ in _); clearbody H';
+                       specialize_by eauto;
+                       move H' at bottom
+                end.
+        all:cbn [denote_symbolic_expr] in *.
+        all:try match goal with |- _ <= _ -> _ => intro end.
+        all:try match goal with
+                | [ H : context[nth_error _ (?x - ?y)] |- _ ]
+                  => rewrite (not_le_minus_0 x y) in H by omega
+                end.
+        move s0 at bottom.
+
+
+        SearchAbout (_ - _ = 0).
+
+        { eapply denote_symbolic_expr_flatten_binding_list; eauto.
+                  all:try solve [ repeat first [ progress subst
+                                       | progress inversion_option
+                                       | progress intros *
+                                       | progress cbn [eq_rect eq_rec eq_ind]
+                                       | solve [ eauto using interpf_flatten_binding_list, denote_symbolic_expr_flatten_binding_list ]
+                                       | progress destruct_head'_or
+                                       | rewrite !(fun var => @lookupb_extendb_full flat_type _ symbolic_expr _ var _ SymbolicExprContextOk)
+                                       | setoid_rewrite in_app_iff
+                                       | break_innermost_match_step
+                                       | progress simpl in *
+                                       | discriminate
+                                       | assumption
+                                       | symmetry; assumption
+                                       | reflexivity
+                                       | progress intros
+                                       | match goal with
+                                         | [ H : ?x = Some ?a, H' : ?x = Some ?b |- _ ]
+                                           => assert (a = b) by (clear -H H'; congruence);
+                                              (subst a || subst b)
+                                         | [ H : ?x <> ?x |- _ ] => exfalso; apply H; clear
+                                         | [ H : lookupb ?t ?m ?n = Some _ |- None = @lookupb _ _ _ ?C ?t' ?m ?n ]
+                                           => let H' := fresh in
+                                              let RHS := match goal with |- _ = ?RHS => RHS end in
+                                              destruct RHS eqn:H'; [ | reflexivity ]
+                                         | [ Hm_small : forall t k, length ?m <= k -> lookupb ?m (SVar k) = None, H : lookupb ?m (SVar ?k') = Some _ |- _ ]
+                                           => rewrite Hm_small in H by omega
+                                         | [ H : lookupb ?t ?m ?n = Some _, H' : lookupb ?t' ?m ?n = Some _ |- _ ]
+                                           => let H'' := fresh in
+                                              pose proof (@lookupb_unique_type _ _ _ _ SymbolicExprContextOk m n t t') as H'';
+                                              rewrite H, H' in H'';
+                                              specialize_by congruence;
+                                              (subst t || subst t')
+                                         | [ H : lookupb ?m ?s = Some ?k, H' : denote_symbolic_expr ?m _ ?s = Some ?k', Hm : forall t sv v, lookupb ?m sv = Some v -> denote_symbolic_expr ?m t sv = Some v |- _ ]
+                                           => let H'' := fresh in
+                                              pose proof (Hm _ _ _ H) as H'';
+                                              rewrite H' in H''; inversion_option;
+                                              (subst k || subst k')
+                                         | [ H : lookupb ?t ?m ?s = Some ?k, H' : denote_symbolic_expr ?m ?t' ?s = Some ?k', Hm : forall T sv v, lookupb ?m sv = Some v -> denote_symbolic_expr ?m T sv = Some v |- _ ]
+                                           => let H'' := fresh in
+                                              let H''' := fresh in
+                                              pose proof (Hm _ _ _ H) as H'';
+                                              pose proof (denote_symbolic_expr_two_types m t t' s) as H''';
+                                              rewrite H', H'' in H''';
+                                              specialize_by congruence;
+                                              (subst t || subst t')
+                                         | [ |- denote_symbolic_expr ?m ?t ?e = Some ?v ]
+                                           => lazymatch m with
+                                              | extendb ?m' _ _
+                                                => apply (fun pf1 => denote_symbolic_expr_weaken m' m pf1 t e v); [ intros ??? | ]
+                                              end
+                                         end ]
+                        | repeat first [ progress cbn [denote_symbolic_expr fst snd projT1 projT2]
+                                       | setoid_rewrite length_extendb
+                                       | rewrite Nat.sub_diag
+                                       | reflexivity
+                                       | discriminate
+                                       | rewrite eq_trans_sym_inv_r
+                                       | progress simpl @nth_error
+                                       | progress unfold var_cast;
+                                         break_innermost_match
+                                       | match goal with
+                                         | [ H : context[flat_type_beq _ _ ?x ?x] |- _ ]
+                                           => setoid_rewrite (flat_type_dec_lb _ _ base_type_code_lb x x eq_refl) in H
+                                         end ] ].
+                  Focus 2.
+                  { cbn [denote_symbolic_expr].
+
+
+          repeat first [ progress subst
+                       | progress inversion_option
+                       | progress intros *
+                       | progress cbn [eq_rect eq_rec eq_ind]
+                       | solve [ eauto using interpf_flatten_binding_list, denote_symbolic_expr_flatten_binding_list ]
+                       | progress destruct_head'_or
+                       | rewrite !(fun var => @lookupb_extendb_full flat_type _ symbolic_expr _ var _ SymbolicExprContextOk)
+                       | setoid_rewrite in_app_iff
+                       | break_innermost_match_step
+                       | progress simpl in *
+                       | discriminate
+                       | assumption
+                       | symmetry; assumption
+                       | reflexivity
+                       | progress intros
+                       | match goal with
+                         | [ H : ?x = Some ?a, H' : ?x = Some ?b |- _ ]
+                           => assert (a = b) by (clear -H H'; congruence);
+                              (subst a || subst b)
+                         | [ H : ?x <> ?x |- _ ] => exfalso; apply H; clear
+                         | [ H : lookupb ?t ?m ?n = Some _ |- None = @lookupb _ _ _ ?C ?t' ?m ?n ]
+                           => let H' := fresh in
+                              let RHS := match goal with |- _ = ?RHS => RHS end in
+                              destruct RHS eqn:H'; [ | reflexivity ]
+                         | [ Hm_small : forall t k, length ?m <= k -> lookupb ?m (SVar k) = None, H : lookupb ?m (SVar ?k') = Some _ |- _ ]
+                           => rewrite Hm_small in H by omega
+                         | [ H : lookupb ?t ?m ?n = Some _, H' : lookupb ?t' ?m ?n = Some _ |- _ ]
+                           => let H'' := fresh in
+                              pose proof (@lookupb_unique_type _ _ _ _ SymbolicExprContextOk m n t t') as H'';
+                              rewrite H, H' in H'';
+                              specialize_by congruence;
+                              (subst t || subst t')
+                         | [ H : lookupb ?m ?s = Some ?k, H' : denote_symbolic_expr ?m _ ?s = Some ?k', Hm : forall t sv v, lookupb ?m sv = Some v -> denote_symbolic_expr ?m t sv = Some v |- _ ]
+                           => let H'' := fresh in
+                              pose proof (Hm _ _ _ H) as H'';
+                              rewrite H' in H''; inversion_option;
+                              (subst k || subst k')
+                         | [ H : lookupb ?t ?m ?s = Some ?k, H' : denote_symbolic_expr ?m ?t' ?s = Some ?k', Hm : forall T sv v, lookupb ?m sv = Some v -> denote_symbolic_expr ?m T sv = Some v |- _ ]
+                           => let H'' := fresh in
+                              let H''' := fresh in
+                              pose proof (Hm _ _ _ H) as H'';
+                              pose proof (denote_symbolic_expr_two_types m t t' s) as H''';
+                              rewrite H', H'' in H''';
+                              specialize_by congruence;
+                              (subst t || subst t')
+                         | [ |- denote_symbolic_expr ?m ?t ?e = Some ?v ]
+                           => lazymatch m with
+                              | extendb ?m' _ _
+                                => apply (fun pf1 => denote_symbolic_expr_weaken m' m pf1 t e v); [ intros ??? | ]
+                              end
+                         end ].
+
+
+                                  | match goal with
+                                      | [ |- context[match eq_trans ?p (eq_sym ?p) with _ => _ end] ]
+                                        => generalize p; unfold eq_sym
+                                      end ] ].
+                    SearchAbout (eq_trans _ (eq_sym _)).
+                    simpl.
+                    unfold var_cast.
+                    break_innermost_match.
+                    Focus 2.
+                    destruct m.
+                    { simpl in *.
+                      setoid_rewrite (@lookupb_empty _ _ _ _ SymbolicExprContextOk) in Heqo0.
+                      congruence. }
+                    { unfold var_cast.
+                      break_innermost_match.
+                      move s at bottom.
+                      unfold lookupb in *; simpl in *.
+                      { break_innermost_match_hyps.
+                        simpl in *.
+                        move p at bottom.
+                      unfold lookup
+                    simpl @extendb.
+                    SearchAbout (?x - ?x).
+                    simpl.
+            [ assumption | | eassumption ].
+            simpl.
+            Focus 2;
+            eauto.
+            eauto.
+          move x at bottom.
+          unfold symbolicify_smart_var in H2.
+          simpl in H2.
+          {
+            match goal with
+            | [ H : _ |- _ ] => apply H
+            end.
+            all:repeat first [ progress subst
+                             | progress inversion_option
+                             | progress intros *
+                             | progress cbn [eq_rect eq_rec eq_ind]
+                             | solve [ eauto using interpf_flatten_binding_list, denote_symbolic_expr_flatten_binding_list ]
+                             | progress destruct_head'_or
+                             | rewrite !(fun var => @lookupb_extendb_full flat_type _ symbolic_expr _ var _ SymbolicExprContextOk)
+                             | setoid_rewrite in_app_iff
+                             | break_innermost_match_step
+                             | progress simpl in *
+                             | discriminate
+                             | assumption
+                             | symmetry; assumption
+                             | reflexivity
+                             | progress intros
+                             | match goal with
+                               | [ H : ?x = Some ?a, H' : ?x = Some ?b |- _ ]
+                                 => assert (a = b) by (clear -H H'; congruence);
+                                    (subst a || subst b)
+                               | [ H : ?x <> ?x |- _ ] => exfalso; apply H; clear
+                               | [ H : lookupb ?t ?m ?n = Some _ |- None = @lookupb _ _ _ ?C ?t' ?m ?n ]
+                                 => let H' := fresh in
+                                    let RHS := match goal with |- _ = ?RHS => RHS end in
+                                    destruct RHS eqn:H'; [ | reflexivity ]
+                               | [ H : lookupb ?t ?m ?n = Some _, H' : lookupb ?t' ?m ?n = Some _ |- _ ]
+                                 => let H'' := fresh in
+                                    pose proof (@lookupb_unique_type _ _ _ _ SymbolicExprContextOk m n t t') as H'';
+                                    rewrite H, H' in H'';
+                                    specialize_by congruence;
+                                    (subst t || subst t')
+                               | [ H : lookupb ?m ?s = Some ?k, H' : denote_symbolic_expr ?m _ ?s = Some ?k', Hm : forall t sv v, lookupb ?m sv = Some v -> denote_symbolic_expr ?m t sv = Some v |- _ ]
+                                 => let H'' := fresh in
+                                    pose proof (Hm _ _ _ H) as H'';
+                                    rewrite H' in H''; inversion_option;
+                                    (subst k || subst k')
+                               | [ H : lookupb ?t ?m ?s = Some ?k, H' : denote_symbolic_expr ?m ?t' ?s = Some ?k', Hm : forall T sv v, lookupb ?m sv = Some v -> denote_symbolic_expr ?m T sv = Some v |- _ ]
+                                 => let H'' := fresh in
+                                    let H''' := fresh in
+                                    pose proof (Hm _ _ _ H) as H'';
+                                    pose proof (denote_symbolic_expr_two_types m t t' s) as H''';
+                                    rewrite H', H'' in H''';
+                                    specialize_by congruence;
+                                    (subst t || subst t')
+                               (*| [ |- denote_symbolic_expr ?m ?t ?e = _ ]
+                                 => lazymatch m with
+                                    | extendb ?m' _ _
+                                      => etransitivity;
+                                         [ apply (fun pf1 => denote_symbolic_expr_Proper m m' pf1 t e e eq_refl); intros ??
+                                         | ]
+                                    end*)
+                               end ].
+            all:repeat match goal with
+                       | [ |- denote_symbolic_expr ?m ?t ?e = Some ?v ]
+                         => lazymatch m with
+                            | extendb ?m' _ _
+                              => apply (fun pf1 => denote_symbolic_expr_weaken m' m pf1 t e v); [ intros ??? | ]
+                            end
+                       end.
+            all:try solve [ repeat first [ progress subst
+                             | progress inversion_option
+                             | progress intros *
+                             | progress cbn [eq_rect eq_rec eq_ind]
+                             | solve [ eauto using interpf_flatten_binding_list, denote_symbolic_expr_flatten_binding_list ]
+                             | progress destruct_head'_or
+                             | rewrite !(fun var => @lookupb_extendb_full flat_type _ symbolic_expr _ var _ SymbolicExprContextOk)
+                             | setoid_rewrite in_app_iff
+                             | break_innermost_match_step
+                             | progress simpl in *
+                             | discriminate
+                             | assumption
+                             | symmetry; assumption
+                             | reflexivity
+                             | progress intros
+                             | match goal with
+                               | [ H : ?x = Some ?a, H' : ?x = Some ?b |- _ ]
+                                 => assert (a = b) by (clear -H H'; congruence);
+                                    (subst a || subst b)
+                               | [ H : ?x <> ?x |- _ ] => exfalso; apply H; clear
+                               | [ H : lookupb ?t ?m ?n = Some _ |- None = @lookupb _ _ _ ?C ?t' ?m ?n ]
+                                 => let H' := fresh in
+                                    let RHS := match goal with |- _ = ?RHS => RHS end in
+                                    destruct RHS eqn:H'; [ | reflexivity ]
+                               | [ H : lookupb ?t ?m ?n = Some _, H' : lookupb ?t' ?m ?n = Some _ |- _ ]
+                                 => let H'' := fresh in
+                                    pose proof (@lookupb_unique_type _ _ _ _ SymbolicExprContextOk m n t t') as H'';
+                                    rewrite H, H' in H'';
+                                    specialize_by congruence;
+                                    (subst t || subst t')
+                               | [ H : lookupb ?m ?s = Some ?k, H' : denote_symbolic_expr ?m _ ?s = Some ?k', Hm : forall t sv v, lookupb ?m sv = Some v -> denote_symbolic_expr ?m t sv = Some v |- _ ]
+                                 => let H'' := fresh in
+                                    pose proof (Hm _ _ _ H) as H'';
+                                    rewrite H' in H''; inversion_option;
+                                    (subst k || subst k')
+                               | [ H : lookupb ?t ?m ?s = Some ?k, H' : denote_symbolic_expr ?m ?t' ?s = Some ?k', Hm : forall T sv v, lookupb ?m sv = Some v -> denote_symbolic_expr ?m T sv = Some v |- _ ]
+                                 => let H'' := fresh in
+                                    let H''' := fresh in
+                                    pose proof (Hm _ _ _ H) as H'';
+                                    pose proof (denote_symbolic_expr_two_types m t t' s) as H''';
+                                    rewrite H', H'' in H''';
+                                    specialize_by congruence;
+                                    (subst t || subst t')
+                               (*| [ |- denote_symbolic_expr ?m ?t ?e = _ ]
+                                 => lazymatch m with
+                                    | extendb ?m' _ _
+                                      => etransitivity;
+                                         [ apply (fun pf1 => denote_symbolic_expr_Proper m m' pf1 t e e eq_refl); intros ??
+                                         | ]
+                                    end*)
+                               end ] ]. } }
+        {
+            eapply ; eauto.
+            Locate interpf_flatten_binding_list.
+
+
+            pose interpf_flatten_binding_list.
+            apply HG2.
+            eauto using interpf_flatten_binding_list.
+            all:repeat first [ progress subst
+                             | progress inversion_option
+                             | progress intros *
+                             | progress cbn [eq_rect eq_rec eq_ind]
+                             | solve [ eauto using interpf_flatten_binding_list, denote_symbolic_expr_flatten_binding_list ]
+                             | progress destruct_head'_or
+                             | rewrite !(fun var => @lookupb_extendb_full flat_type _ symbolic_expr _ var _ SymbolicExprContextOk)
+                             | setoid_rewrite in_app_iff
+                             | break_innermost_match_step
+                             | progress simpl in *
+                             | discriminate
+                             | assumption
+                             | symmetry; assumption
+                             | reflexivity
+                             | progress intros
+                             | match goal with
+                               | [ H : ?x = Some ?a, H' : ?x = Some ?b |- _ ]
+                                 => assert (a = b) by (clear -H H'; congruence);
+                                    (subst a || subst b)
+                               | [ H : ?x <> ?x |- _ ] => exfalso; apply H; clear
+                               | [ H : lookupb ?t ?m ?n = Some _ |- None = @lookupb _ _ _ ?C ?t' ?m ?n ]
+                                 => let H' := fresh in
+                                    let RHS := match goal with |- _ = ?RHS => RHS end in
+                                    destruct RHS eqn:H'; [ | reflexivity ]
+                               | [ H : lookupb ?t ?m ?n = Some _, H' : lookupb ?t' ?m ?n = Some _ |- _ ]
+                                 => let H'' := fresh in
+                                    pose proof (@lookupb_unique_type _ _ _ _ SymbolicExprContextOk m n t t') as H'';
+                                    rewrite H, H' in H'';
+                                    specialize_by congruence;
+                                    (subst t || subst t')
+                               | [ H : lookupb ?m ?s = Some ?k, H' : denote_symbolic_expr ?m _ ?s = Some ?k', Hm : forall t sv v, lookupb ?m sv = Some v -> denote_symbolic_expr ?m t sv = Some v |- _ ]
+                                 => let H'' := fresh in
+                                    pose proof (Hm _ _ _ H) as H'';
+                                    rewrite H' in H''; inversion_option;
+                                    (subst k || subst k')
+                               | [ H : lookupb ?t ?m ?s = Some ?k, H' : denote_symbolic_expr ?m ?t' ?s = Some ?k', Hm : forall T sv v, lookupb ?m sv = Some v -> denote_symbolic_expr ?m T sv = Some v |- _ ]
+                                 => let H'' := fresh in
+                                    let H''' := fresh in
+                                    pose proof (Hm _ _ _ H) as H'';
+                                    pose proof (denote_symbolic_expr_two_types m t t' s) as H''';
+                                    rewrite H', H'' in H''';
+                                    specialize_by congruence;
+                                    (subst t || subst t')
+                               (*| [ |- denote_symbolic_expr ?m ?t ?e = _ ]
+                                 => lazymatch m with
+                                    | extendb ?m' _ _
+                                      => etransitivity;
+                                         [ apply (fun pf1 => denote_symbolic_expr_Proper m m' pf1 t e e eq_refl); intros ??
+                                         | ]
+                                    end*)
+                               end ].
+            move H1 at bottom.
+            lazymatch goal with
+                               | [ H : lookupb ?t ?m ?s = Some ?k, H' : denote_symbolic_expr ?m ?t' ?s = Some ?k', Hm : forall t sv v, lookupb ?m sv = Some v -> denote_symbolic_expr ?m t sv = Some v |- _ ]
+                                 => let H'' := fresh in
+                                    let H''' := fresh in
+                                    pose proof (Hm _ _ _ H) as H'';
+                                    pose proof (denote_symbolic_expr_two_types m t t' s) as H''';
+                                    rewrite ?H', ?H'' in H''';
+                                    specialize_by congruence;
+                                    try (subst t || subst t')
+                                      end.
+            apply Hm in H4.
+            all:admit. } }
+              move m at bottom.
+              move t0 at bottom.
+
+          }
+
+        {
+
+
+            lazymatch goal with
+            end.
+                     lazymatch goal with
+                     | [ |- lookupb (extendb ?m _ _) _ = lookupb ?m' _ ]
+                       => unify m m'
+                     end
+                   | ]
+            end.
+              repeat first [ rewrite !(fun var => @lookupb_extendb_full flat_type _ symbolic_expr _ var _ SymbolicExprContextOk)
+                           | progress subst
+                           | break_innermost_match_step          match goal with
+          | [ H : lookupb ?m ?s = Some ?k, H' : denote_symbolic_expr ?m _ ?s = Some ?k', Hm : forall t sv v, lookupb ?m sv = Some v -> denote_symbolic_expr ?m t sv = Some v |- _ ]
+            => let H'' := fresh in
+               pose proof (Hm _ _ _ H) as H'';
+                 rewrite H' in H''; inversion_option;
+                   (subst k || subst k')
+          end .
+          solve [ eauto using interpf_flatten_binding_list, denote_symbolic_expr_flatten_binding_list ].
+Focus 2.
+          { eauto. lazymatch goal with
+            | [ H : lookupb ?m ?s = Some ?k, H' : denote_symbolic_expr ?m _ ?s = Some ?k', Hm : forall t sv v, lookupb ?m sv = Some v -> denote_symbolic_expr ?m t sv = Some v |- _ ]
+              => let H'' := fresh in
+                 pose proof (Hm _ _ _ H) as H'';
+                   rewrite H' in H''; inversion_option;
+                     (subst k || subst k')
+            end.
+
+          { eapply HG2.
+            eapply HGm.
+            eassumption.
+            match goal with
+            end.
+            move s at bottom.
+            pose proof
+          2:etransitivity;
+            [ eapply denote_symbolic_expr_Proper;
+              [ intros ?? | reflexivity ];
+              lazymatch goal with
+              | [ |- lookupb (extendb ?m _ _) _ = lookupb ?m' _ ]
+                => unify m m'
+              end;
+              repeat first [ rewrite !(fun var => @lookupb_extendb_full flat_type _ symbolic_expr _ var _ SymbolicExprContextOk)
+                           | progress subst
+                           | progress simpl in *
+                           | congruence
+                           | break_innermost_match_step
+                           | match goal with
+                             | [ H : lookupb ?t ?m ?n = Some _ |- None = @lookupb _ _ _ ?C ?t' ?m ?n ]
+                               => let H' := fresh in
+                                  let RHS := match goal with |- _ = ?RHS => RHS end in
+                                  destruct RHS eqn:H'; [ | reflexivity ]
+                             | [ H : lookupb ?t ?m ?n = Some _, H' : lookupb ?t' ?m ?n = Some _ |- _ ]
+                               => let H'' := fresh in
+                                  pose proof (@lookupb_unique_type _ _ _ _ SymbolicExprContextOk m n t t') as H'';
+                                  rewrite H, H' in H'';
+                                  specialize_by congruence;
+                                  (subst t || subst t')
+                             end ]
+            | ].
+            | solve [ eauto ] ].
+
+          { intros ??.
+              instantiate (1:=m).
+
+              break_innermost_match; subst; simpl; try congruence.
+              lazymatch goal with
+              end.
+              congruence. }
+            reflexivity.
+            { eauto. } }
+          Unfocus.
+          Focus 2.
+          {
+
+
+              SearchAbout lookupb_removeb_different.
+              Set Printing Implicit.
+                reflexivity.
+              rewrite look
+
+
+          Focus 3.
+          Focus 2.
+          Focus 2.
+          { right; eapply HGm; [ | eassumption ].
+
+          2:eauto.
+          2:
+        Focus 2.
+        { cbn [interpf interpf_step LetIn.Let_In].
+          rewrite_hyp * by eauto.
+          match goal with
+          | [ H : _ |- _ ] => apply H
+          end.
+          all:intros *.
+          all:try solve [ repeat first [ rewrite !(fun var => @lookupb_extendb_full flat_type _ symbolic_expr _ var _ SymbolicExprContextOk)
+                         | setoid_rewrite in_app_iff
+                         | progress subst
+                         | progress simpl in *
+                         | progress inversion_prod
+                         | progress inversion_option
+                         | progress destruct_head or
+                         | solve [ eauto using interpf_flatten_binding_list, denote_symbolic_expr_flatten_binding_list ]
+                         | progress intros ] ].
+          Focus 3.
+          { repeat first [ rewrite !(fun var => @lookupb_extendb_full flat_type _ symbolic_expr _ var _ SymbolicExprContextOk)
+                         | setoid_rewrite in_app_iff
+                         | progress subst
+                         | progress simpl in *
+                         | progress inversion_prod
+                         | progress inversion_option
+                         | progress destruct_head or
+                         | solve [ eauto using interpf_flatten_binding_list, denote_symbolic_expr_flatten_binding_list ]
+                         | progress intros
+                         | match goal with
+                           | [ H : nth_error ?ls (length ?ls) = Some _ |- _ ]
+                             => rewrite (proj2 (nth_error_None _ _)) in H by reflexivity
+                           end
+                         | break_innermost_match_hyps_step
+                         | break_innermost_match_step
+                         | progress break_match_hyps ].
+            Focus 4.
+            { move m at bottom.
+              destruct m; simpl in *; [ | congruence ].
+              specialize_by_assumption.
+              specialize (IHHwf nil).
+              specialize_by_assumption.
+              clear H2 Heqo0.
+              clear Hm.
+              simpl in *.
+              clear HGm.
+              move Heqo at bottom.
+              unfold norm_symbolize_exprf in Heqo.
+              move e1 at bottom.
+              unfold option_map in
+              move G at bottom.
+              move G at bottom.
+              unfold lookupb in Hm.
+              unfold SymbolicExprContext in Hm.
+              unfold AListContext in Hm.
+              unfold find in Hm.
+              clear Hm.
+            SearchAbout (
+
+            Set Printing Implicit.
+            break_innermost_match_hyps.
+          { repeat first [ rewrite !(fun var => @lookupb_extendb_full flat_type _ symbolic_expr _ var _ SymbolicExprContextOk)
+                         | setoid_rewrite in_app_iff ].
+                         |
+
+          repeat first [
+                       | setoid_rewrite in_app_iff
+                       | progress break_innermost_match
+                       | progress subst
+                       | progress simpl in *
+                       | progress inversion_prod
+                       | progress inversion_option
+                       | progress destruct_head or
+                       | solve [ eauto using interpf_flatten_binding_list, denote_symbolic_expr_flatten_binding_list ]
+                       | progress intros ].
+          unfold LetIn.Let_In.
+          simpl.
+        match goal with
+        | [ H : norm_symbolize_exprf _ = Some _ |- _ ]
+        end
+      { break_innermost_match.
+        { apply H0.
+        all:try match goal with
+                | [ H : context[interpf interp_op (csef _ _)] |- _ ] => erewrite H; [ reflexivity | | eauto | eauto ]
+                end;
+          intros *;
+          repeat first [ rewrite !(fun var => @lookupb_extendb_full flat_type _ symbolic_expr _ var _ SymbolicExprContextOk)
+                       | setoid_rewrite in_app_iff
+                       | progress break_innermost_match
+                       | progress subst
+                       | progress simpl in *
+                       | progress inversion_prod
+                       | progress inversion_option
+                       | progress destruct_head or
+                       | solve [ eauto using interpf_flatten_binding_list, denote_symbolic_expr_flatten_binding_list ]
+                       | progress intros ].
+        w
+        3:rewrite_hyp !* by eauto.
+        5:rewrite_hyp !* by eauto.
+        6:rewrite_hyp !* by eauto.
+        lazymatch goal with
+        | [ Hm : forall t e1 e2 s v, symbolize_exprf _ = _ -> _, H' : symbolize_exprf _ = _ |- _ ]
+                => erewrite (Hm _ _ _ _ _ H') by eassumption
+              end.
             [ match goal with
               | [ Hm : forall t e1 e2 s v, symbolize_exprf _ = _ -> _, H' : symbolize_exprf _ = _ |- _ ]
                 => erewrite (Hm _ _ _ _ _ H') by eassumption
@@ -174,12 +1854,12 @@ Section symbolic.
                          | progress inversion_prod
                          | progress inversion_option
                          | progress destruct_head or
-                         | solve [ eauto using interpf_flatten_binding_list ]
+                         | solve [ eauto using interpf_flatten_binding_list, denote_symbolic_expr_flatten_binding_list ]
                          | progress intros ] ].
         admit.
         admit.
         admit. }*)
-  Admitted.
+  Abort.
 
   Lemma interpf_prepend_prefix t e prefix
     : interpf interp_op (@prepend_prefix _ t e prefix) = interpf interp_op e.
@@ -193,13 +1873,13 @@ Section symbolic.
   Proof.
     destruct Hwf; simpl; intros.
     etransitivity; [ | eapply interpf_prepend_prefix ].
-    eapply interpf_csef; eauto;
+    (*eapply interpf_csef; eauto;
       [ ..
       | eapply wff_prepend_prefix; [ .. | solve [ eauto ] ] ].
     { intros; eapply interpf_flatten_binding_list; eassumption. }
     { admit. }
-    { admit. }
-  Admitted.
+    { admit. }*)
+  Abort.
 
   Lemma InterpCSE t (e : Expr t)
         (prefix : forall var, list (sigT (fun t : flat_type => @exprf var t)))
@@ -211,8 +1891,8 @@ Section symbolic.
         (Hwf : Wf e)
     : forall x, Interp interp_op (@CSE t e prefix) x = Interp interp_op e x.
   Proof.
-    apply interp_cse; auto.
-  Qed.
+    admit; apply interp_cse; auto.
+  Abort.
 End symbolic.
 
 Hint Rewrite @InterpCSE using solve_wf_side_condition : reflective_interp.
